infoflow: general cleanup
Signed-off-by: Ryan Barry <ryan.barry@unsw.edu.au>

proof/infoflow/Noninterference_Base.thy
@@ -19,69 +19,66 @@ text \<open>
 section \<open>Generic systems\<close>
 
 lemma un_eq:
-  "\<lbrakk>S = S'; T = T'\<rbrakk> \<Longrightarrow> S \<union> T = S' \<union> T'"
+  "\<lbrakk> S = S'; T = T' \<rbrakk> \<Longrightarrow> S \<union> T = S' \<union> T'"
   by auto
 
 lemma Un_eq:
-  "\<lbrakk>\<And> x y. \<lbrakk>x \<in> xs; y \<in> ys\<rbrakk> \<Longrightarrow> P x = Q y; \<exists> x. x \<in> xs; \<exists> y. y \<in> ys\<rbrakk>
-    \<Longrightarrow> (\<Union>x\<in>xs. P x) = (\<Union>y\<in>ys. Q y)"
+  "\<lbrakk> \<And>x y. \<lbrakk> x \<in> xs; y \<in> ys \<rbrakk> \<Longrightarrow> P x = Q y; \<exists>x. x \<in> xs; \<exists>y. y \<in> ys \<rbrakk>
+     \<Longrightarrow> (\<Union>x \<in> xs. P x) = (\<Union>y \<in> ys. Q y)"
   by auto
 
 lemma Int_eq:
-  "\<lbrakk>\<And> x y. \<lbrakk>x \<in> xs; y \<in> ys\<rbrakk> \<Longrightarrow> P x = Q y; \<exists> x. x \<in> xs; \<exists> y. y \<in> ys\<rbrakk>
-    \<Longrightarrow> (\<Inter>x\<in>xs. P x) = (\<Inter>y\<in>ys. Q y)"
+  "\<lbrakk> \<And>x y. \<lbrakk> x \<in> xs; y \<in> ys \<rbrakk> \<Longrightarrow> P x = Q y; \<exists>x. x \<in> xs; \<exists>y. y \<in> ys \<rbrakk>
+     \<Longrightarrow> (\<Inter>x \<in> xs. P x) = (\<Inter>y \<in> ys. Q y)"
   by auto
 
 lemma Un_eq_Int:
-  assumes ex: "\<exists> x. x \<in> xs"
-  assumes ey: "\<exists> y. y \<in> ys"
-  assumes a: "\<And> x y. \<lbrakk>x \<in> xs; y \<in> ys\<rbrakk> \<Longrightarrow> S x = S' y"
-  shows "(\<Union>x\<in>xs. S x) = (\<Inter>x\<in>ys. S' x)"
-  apply(rule equalityI)
-   apply(clarsimp)
-   apply(drule a, assumption, simp)
+  assumes ex: "\<exists>x. x \<in> xs"
+  assumes ey: "\<exists>y. y \<in> ys"
+  assumes a: "\<And>x y. \<lbrakk> x \<in> xs; y \<in> ys \<rbrakk> \<Longrightarrow> S x = S' y"
+  shows "(\<Union>x \<in> xs. S x) = (\<Inter>x \<in> ys. S' x)"
+  apply (rule equalityI)
+   apply (clarsimp)
+   apply (drule a, assumption, simp)
   apply clarsimp
-  apply(insert ex ey)
+  apply (insert ex ey)
   apply clarsimp
-  apply(frule a, assumption)
+  apply (frule a, assumption)
   apply fastforce
   done
+
 
 subsection\<open>Run function\<close>
 
-primrec Run :: "('e \<Rightarrow> ('s \<times> 's) set) \<Rightarrow> 'e list \<Rightarrow> ('s \<times> 's) set"
-where
-  "Run Stepf []     = Id" |
-  "Run Stepf (a#as) = Stepf a O Run Stepf as"
+primrec Run :: "('e \<Rightarrow> ('s \<times> 's) set) \<Rightarrow> 'e list \<Rightarrow> ('s \<times> 's) set" where
+  "Run Stepf []     = Id"
+| "Run Stepf (a#as) = Stepf a O Run Stepf as"
 
 
 lemma Run_mid[rule_format]:
-  shows
-  "(s,u) \<in> Run Stepf (as @ bs) \<longrightarrow> (\<exists> t. (s,t) \<in> Run Stepf as \<and> (t,u) \<in> Run Stepf bs)"
-  proof(induct as arbitrary: s u bs)
+  "(s,u) \<in> Run Stepf (as @ bs) \<longrightarrow> (\<exists>t. (s,t) \<in> Run Stepf as \<and> (t,u) \<in> Run Stepf bs)"
+proof (induct as arbitrary: s u bs)
   case Nil show ?case
-   apply(clarsimp)
-   done
-  next
+    by (clarsimp)
+next
   case (Cons a as) show ?case
-  apply(clarsimp simp: relcomp_def)
-  apply(drule "Cons.hyps"[rule_format])
-  apply fastforce
-  done
+    apply (clarsimp simp: relcomp_def)
+    apply (drule "Cons.hyps"[rule_format])
+    apply fastforce
+    done
 qed
 
 lemma Run_trans:
-  "\<lbrakk>(s,t) \<in> Run Stepf as; (t,u) \<in> Run Stepf bs\<rbrakk> \<Longrightarrow> (s,u) \<in> Run Stepf (as @ bs)"
+  "\<lbrakk> (s,t) \<in> Run Stepf as; (t,u) \<in> Run Stepf bs \<rbrakk>
+     \<Longrightarrow> (s,u) \<in> Run Stepf (as @ bs)"
   by (induct as arbitrary: bs s t u) auto
 
 lemma Run_app:
   "Run Stepf (as @ bs) = (Run Stepf as) O (Run Stepf bs)"
-  apply(rule equalityI)
-   apply(fastforce dest: Run_mid)
-  apply(fastforce intro: Run_trans)
+  apply (rule equalityI)
+   apply (fastforce dest: Run_mid)
+  apply (fastforce intro: Run_trans)
   done
-
-
 
 
 subsection \<open>Base system locale\<close>
@@ -93,28 +90,25 @@ locale system =
 begin
 
 (* State 's' is reachable from the initial state 's0'. *)
-definition reachable
-where
-  "reachable s \<equiv> \<exists> js. s \<in> execution A s0 js"
+definition reachable where
+  "reachable s \<equiv> \<exists>js. s \<in> execution A s0 js"
 
-definition Step
-where
+definition Step where
   "Step a \<equiv> {(s,s') . s' \<in> execution A s [a]}"
 
 (* The system is "observationally deterministic": that is, the
  * observable part of the system is always deterministic. *)
-definition obs_det
-where
-  "obs_det \<equiv> \<forall> s js. (\<exists> s'. execution A s js = {s'})"
+definition obs_det where
+  "obs_det \<equiv> \<forall>s js. (\<exists>s'. execution A s js = {s'})"
 
 lemmas obs_detD = obs_det_def[THEN meta_eq_to_obj_eq, THEN iffD1, rule_format]
 
 (* The abstraction/concretisation functions "Init"/"Fin"
  * don't abstract away information. *)
-definition no_abs
-where
-  "no_abs \<equiv> \<forall> x s as . reachable s \<longrightarrow> x \<in> steps (Simulation.Step A) (Init A s) as
-                        \<longrightarrow> Init A (Fin A x) = {x}"
+definition no_abs where
+  "no_abs \<equiv> \<forall>x s as . reachable s
+                       \<longrightarrow> x \<in> steps (Simulation.Step A) (Init A s) as
+                       \<longrightarrow> Init A (Fin A x) = {x}"
 
 lemmas no_absD = no_abs_def[THEN meta_eq_to_obj_eq, THEN iffD1, rule_format]
 
@@ -130,21 +124,21 @@ text\<open>
   is always an enabled transition from every reachable state.\<close>
 
 locale enabled_system = system +
-  assumes enabled: "(\<exists> js. s \<in> execution A s0 js) \<Longrightarrow> \<exists> s'. s' \<in> execution A s js"
+  assumes enabled: "(\<exists>js. s \<in> execution A s0 js) \<Longrightarrow> \<exists>s'. s' \<in> execution A s js"
 begin
 
 lemma reachable_enabled:
-  "reachable s \<Longrightarrow> \<exists> s'. s' \<in> execution A s js"
-  apply(simp add: reachable_def)
-  apply(erule enabled)
+  "reachable s \<Longrightarrow> \<exists>s'. s' \<in> execution A s js"
+  apply (simp add: reachable_def)
+  apply (erule enabled)
   done
 
 lemma enabled_Step:
-  "reachable s \<Longrightarrow> \<exists> s'. (s,s') \<in> Step a"
-  apply(simp add: Step_def, blast intro: reachable_enabled)
-  done
+  "reachable s \<Longrightarrow> \<exists>s'. (s,s') \<in> Step a"
+  by (simp add: Step_def, blast intro: reachable_enabled)
 
 end
+
 
 subsection \<open>Step system\<close>
 
@@ -164,8 +158,8 @@ begin
 
 lemma execution_Run':
   "s \<in> execution A s0 js \<Longrightarrow> execution A s as = {s'. (s,s') \<in> Run Step as}"
-  apply(rule execution_Run)
-  apply(fastforce simp: reachable_def)
+  apply (rule execution_Run)
+  apply (fastforce simp: reachable_def)
   done
 
 lemma reachable_Run:
@@ -182,33 +176,32 @@ lemma Run_reachable:
   apply blast
   done
 
-
 lemma reachable_execution:
-  "\<lbrakk>reachable s; s' \<in> execution A s js\<rbrakk> \<Longrightarrow> reachable s'"
-  apply(clarsimp simp: reachable_def)
-  apply(rule_tac x="jsa @ js" in exI)
-  apply(frule execution_Run'[where s=s and as=js])
-  apply(simp add: execution_Run[where s=s0, simplified reachable_s0])
-  apply(fastforce simp: Run_app)
+  "\<lbrakk> reachable s; s' \<in> execution A s js \<rbrakk> \<Longrightarrow> reachable s'"
+  apply (clarsimp simp: reachable_def)
+  apply (rule_tac x="jsa @ js" in exI)
+  apply (frule execution_Run'[where s=s and as=js])
+  apply (simp add: execution_Run[where s=s0, simplified reachable_s0])
+  apply (fastforce simp: Run_app)
   done
 
 lemma reachable_Step:
-  "\<lbrakk>reachable s; (s,s') \<in> Step a\<rbrakk> \<Longrightarrow> reachable s'"
-  apply(erule reachable_execution)
-  apply(simp add: Step_def)
+  "\<lbrakk> reachable s; (s,s') \<in> Step a \<rbrakk> \<Longrightarrow> reachable s'"
+  apply (erule reachable_execution)
+  apply (simp add: Step_def)
   done
 
 lemma reachable_induct_helper:
-  assumes a:
-    "\<And>s s' a. \<lbrakk>reachable s; P s; (s, s') \<in> Step a\<rbrakk> \<Longrightarrow> P s'"
-  shows "\<lbrakk>(s0, s1) \<in> Run Step as; P s0\<rbrakk> \<Longrightarrow> P s1"
+  assumes a: "\<And>s s' a. \<lbrakk> reachable s; P s; (s, s') \<in> Step a \<rbrakk> \<Longrightarrow> P s'"
+  shows "\<lbrakk> (s0, s1) \<in> Run Step as; P s0 \<rbrakk> \<Longrightarrow> P s1"
   apply (induct as arbitrary: s1 rule: rev_induct)
    apply simp
-  apply(fastforce dest: Run_mid intro: a Run_reachable)
+  apply (fastforce dest: Run_mid intro: a Run_reachable)
   done
 
 lemma reachable_induct:
-  "\<lbrakk>(\<And>s s' a. reachable s \<Longrightarrow> (s,s') \<in> (Step a) \<Longrightarrow> P s \<Longrightarrow> P s'); reachable s1; P s0\<rbrakk> \<Longrightarrow> P s1"
+  "\<lbrakk> \<And>s s' a. reachable s \<Longrightarrow> (s,s') \<in> (Step a) \<Longrightarrow> P s \<Longrightarrow> P s'; reachable s1; P s0 \<rbrakk>
+     \<Longrightarrow> P s1"
   apply (drule reachable_Run)
   apply (elim exE)
   apply (rule reachable_induct_helper)
@@ -216,6 +209,7 @@ lemma reachable_induct:
   done
 
 end
+
 
 subsection \<open>Init Fin system\<close>
 
@@ -229,90 +223,91 @@ locale Init_Fin_system = system A s0
   for A :: "('a,'s,'e) data_type" and s0 :: "'s"  +
   assumes reachable_s0: "reachable s0"
   assumes Fin_Init: "reachable s \<Longrightarrow> Fin A ` Init A s = {s}"
-  assumes Init_Fin: "reachable s \<Longrightarrow> x \<in> steps (Simulation.Step A) (Init A s) as \<Longrightarrow>  x \<in> Init A (Fin A x)"
+  assumes Init_Fin: "\<lbrakk> reachable s; x \<in> steps (Simulation.Step A) (Init A s) as \<rbrakk>
+                       \<Longrightarrow> x \<in> Init A (Fin A x)"
   assumes obs_det_or_no_abs: "obs_det \<or> no_abs"
 begin
 
-
 lemma execution_subset_Run:
   "reachable s \<Longrightarrow> execution A s as \<subseteq> {s'. (s,s') \<in> Run Step as}"
-  apply(induct as arbitrary: s rule: rev_induct)
-   apply(simp add: execution_def steps_def Fin_Init)
-  apply(simp add: execution_def steps_def)
-  apply(rule subsetI)
+  apply (induct as arbitrary: s rule: rev_induct)
+   apply (simp add: execution_def steps_def Fin_Init)
+  apply (simp add: execution_def steps_def)
+  apply (rule subsetI)
   apply clarsimp
-  apply(rule Run_trans)
+  apply (rule Run_trans)
    apply blast
-  apply(cut_tac x=xc and s=s and as=xs in Init_Fin, (simp add: steps_def)+)
-  apply(clarsimp simp: Step_def execution_def steps_def)
+  apply (cut_tac x=xc and s=s and as=xs in Init_Fin, (simp add: steps_def)+)
+  apply (clarsimp simp: Step_def execution_def steps_def)
   apply blast
   done
 
 lemma Run_subset_execution:
-  "\<lbrakk>no_abs; reachable s\<rbrakk> \<Longrightarrow> {s'. (s,s') \<in> Run Step as} \<subseteq> execution A s as"
-  apply(induct as arbitrary: s rule: rev_induct)
-   apply(simp add: execution_def steps_def Fin_Init)
-  apply(simp add: execution_def steps_def)
-  apply(rule subsetI)
+  "\<lbrakk> no_abs; reachable s \<rbrakk> \<Longrightarrow> {s'. (s,s') \<in> Run Step as} \<subseteq> execution A s as"
+  apply (induct as arbitrary: s rule: rev_induct)
+   apply (simp add: execution_def steps_def Fin_Init)
+  apply (simp add: execution_def steps_def)
+  apply (rule subsetI)
   apply clarsimp
-  apply(drule Run_mid)
+  apply (drule Run_mid)
   apply clarsimp
-  apply(drule_tac x=s in meta_spec)
+  apply (drule_tac x=s in meta_spec)
   apply clarsimp
-  apply(drule_tac subsetD)
+  apply (drule_tac subsetD)
    apply blast
-  apply(clarsimp simp: Image_def image_def Step_def execution_def steps_def)
-  apply(rule_tac x=xc in exI)
+  apply (clarsimp simp: Image_def image_def Step_def execution_def steps_def)
+  apply (rule_tac x=xc in exI)
   apply clarsimp
-  apply(rule_tac x=xd in bexI)
+  apply (rule_tac x=xd in bexI)
    apply assumption
-  apply(drule_tac x=xb in no_absD)
-    apply(simp add: steps_def Image_def)+
+  apply (drule_tac x=xb in no_absD)
+    apply (simp add: steps_def Image_def)+
   done
 
 lemma Run_det:
-  "obs_det \<Longrightarrow> \<exists> s'. {s'. (s,s') \<in> Run Step as} = {s'}"
-  apply(induct as arbitrary: s rule: rev_induct)
+  "obs_det \<Longrightarrow> \<exists>s'. {s'. (s,s') \<in> Run Step as} = {s'}"
+  apply (induct as arbitrary: s rule: rev_induct)
    apply simp
-  apply(simp add: Run_app relcomp_def)
-  apply(drule_tac x=s in meta_spec)
+  apply (simp add: Run_app relcomp_def)
+  apply (drule_tac x=s in meta_spec)
   apply clarsimp
-  apply(drule_tac s=s' and js="[x]" in obs_detD)
+  apply (drule_tac s=s' and js="[x]" in obs_detD)
   apply (clarsimp simp: Step_def)
-  apply(rule_tac x="s'a" in exI)
+  apply (rule_tac x="s'a" in exI)
   apply (auto dest: equalityD1)
   done
 
 lemma eq:
-  "\<lbrakk>S \<subseteq> T; \<exists> x. S = {x}; \<exists> y. T = {y}\<rbrakk> \<Longrightarrow> S = T"
-  apply blast
-  done
+  "\<lbrakk> S \<subseteq> T; \<exists>x. S = {x}; \<exists>y. T = {y} \<rbrakk> \<Longrightarrow> S = T"
+  by blast
 
 lemma execution_Run:
   "reachable s \<Longrightarrow> execution A s as = {s'. (s,s') \<in> Run Step as}"
-  apply(rule disjE[OF obs_det_or_no_abs])
-   apply(rule eq)
-     apply(erule execution_subset_Run)
-    apply(erule obs_detD)
-   apply(erule Run_det)
-  apply(rule equalityI)
-   apply(erule execution_subset_Run)
-  apply(erule (1) Run_subset_execution)
+  apply (rule disjE[OF obs_det_or_no_abs])
+   apply (rule eq)
+     apply (erule execution_subset_Run)
+    apply (erule obs_detD)
+   apply (erule Run_det)
+  apply (rule equalityI)
+   apply (erule execution_subset_Run)
+  apply (erule (1) Run_subset_execution)
   done
 
 end
 
+
 lemma Init_Fin_system_Step_system:
   "Init_Fin_system A s0 \<Longrightarrow> Step_system A s0"
-  apply(unfold_locales)
-   apply(erule Init_Fin_system.reachable_s0)
-  apply(erule (1) Init_Fin_system.execution_Run)
+  apply (unfold_locales)
+   apply (erule Init_Fin_system.reachable_s0)
+  apply (erule (1) Init_Fin_system.execution_Run)
   done
 
 sublocale Init_Fin_system \<subseteq> Step_system
-  apply(rule Init_Fin_system_Step_system)
-  apply(unfold_locales)
+  apply (rule Init_Fin_system_Step_system)
+  apply (unfold_locales)
   done
+
 
 subsection \<open>Init inv Fin system\<close>
 
@@ -334,75 +329,73 @@ locale Init_inv_Fin_system = system A s0
 begin
 
 lemma inv_and_inj: "reachable s \<Longrightarrow> Fin A i = s \<Longrightarrow> Init A s = {i}"
-  using Fin_inj Init_inv_Fin by (blast dest:injD)
+  using Fin_inj Init_inv_Fin by (blast dest: injD)
 
 lemma s0_reachable:
   "reachable s0"
-  apply(simp add: reachable_def)
-  apply(rule_tac x="[]" in exI)
-  apply(simp add: execution_def steps_def)
-  using Fin_Init_s0.
+  apply (simp add: reachable_def)
+  apply (rule_tac x="[]" in exI)
+  apply (simp add: execution_def steps_def)
+  using Fin_Init_s0 .
 
 lemma foldl_foldl_Step:
-  "\<lbrakk>x \<in> foldl (\<lambda>S j. data_type.Step A j `` S) M as;
-   M \<subseteq> foldl (\<lambda>S j. data_type.Step A j `` S) B js\<rbrakk>
-       \<Longrightarrow> x \<in> foldl (\<lambda>S j. data_type.Step A j `` S)
-               (foldl (\<lambda>S j. data_type.Step A j `` S) B js) as"
-  apply(induct  as arbitrary: x M js B rule: rev_induct)
+  "\<lbrakk> x \<in> foldl (\<lambda>S j. data_type.Step A j `` S) M as;
+     M \<subseteq> foldl (\<lambda>S j. data_type.Step A j `` S) B js \<rbrakk>
+     \<Longrightarrow> x \<in> foldl (\<lambda>S j. data_type.Step A j `` S) (foldl (\<lambda>S j. data_type.Step A j `` S) B js) as"
+  apply (induct as arbitrary: x M js B rule: rev_induct)
    apply fastforce
   apply simp
-  apply(erule ImageE)
-  apply(drule_tac x=xb in meta_spec)
-  apply(drule_tac x=M in meta_spec)
+  apply (erule ImageE)
+  apply (drule_tac x=xb in meta_spec)
+  apply (drule_tac x=M in meta_spec)
   apply simp
-  apply(drule_tac x=js in meta_spec)
-  apply(drule_tac x=B in meta_spec, simp)
-  apply(blast)
+  apply (drule_tac x=js in meta_spec)
+  apply (drule_tac x=B in meta_spec, simp)
+  apply (blast)
   done
 
 lemma reachable_Fin:
-  "\<lbrakk>reachable s;
-    x \<in> steps (Simulation.Step A) (Init A s) as\<rbrakk>
-   \<Longrightarrow> reachable (Fin A x)"
-  apply(cut_tac s=s in Init_inv_Fin, assumption)
-  apply(clarsimp simp: reachable_def execution_def steps_def)
-  apply(rule_tac x="js@as" in exI)
-  apply(rule imageI)
-  apply(subgoal_tac "{s'. Fin A s' = Fin A xa} = {xa}")
+  "\<lbrakk> reachable s; x \<in> steps (Simulation.Step A) (Init A s) as \<rbrakk>
+     \<Longrightarrow> reachable (Fin A x)"
+  apply (cut_tac s=s in Init_inv_Fin, assumption)
+  apply (clarsimp simp: reachable_def execution_def steps_def)
+  apply (rule_tac x="js@as" in exI)
+  apply (rule imageI)
+  apply (subgoal_tac "{s'. Fin A s' = Fin A xa} = {xa}")
    apply simp
-   apply(erule foldl_foldl_Step)
+   apply (erule foldl_foldl_Step)
    apply blast
-  apply(blast dest: injD[OF Fin_inj])
+  apply (blast dest: injD[OF Fin_inj])
   done
 
 end
 
+
 lemma Init_inv_Fin_system_Init_Fin_system:
   "Init_inv_Fin_system A s0 \<Longrightarrow> Init_Fin_system A s0"
-  apply(unfold_locales)
-     apply(erule Init_inv_Fin_system.s0_reachable)
-    apply(simp add: Init_inv_Fin_system.Init_inv_Fin)
-    apply(simp add: image_def)
-    apply(fastforce simp: system.reachable_def execution_def)
-   apply(cut_tac s="Fin A x" in Init_inv_Fin_system.Init_inv_Fin)
+  apply (unfold_locales)
+     apply (erule Init_inv_Fin_system.s0_reachable)
+    apply (simp add: Init_inv_Fin_system.Init_inv_Fin)
+    apply (simp add: image_def)
+    apply (fastforce simp: system.reachable_def execution_def)
+   apply (cut_tac s="Fin A x" in Init_inv_Fin_system.Init_inv_Fin)
      apply assumption
-    apply(blast intro: Init_inv_Fin_system.reachable_Fin)
+    apply (blast intro: Init_inv_Fin_system.reachable_Fin)
    apply simp
-  apply(rule disjI2)
-  apply(clarsimp simp: system.no_abs_def)
-  apply(frule Init_inv_Fin_system.Fin_inj)
-  apply(cut_tac s="Fin A x" in Init_inv_Fin_system.Init_inv_Fin)
+  apply (rule disjI2)
+  apply (clarsimp simp: system.no_abs_def)
+  apply (frule Init_inv_Fin_system.Fin_inj)
+  apply (cut_tac s="Fin A x" in Init_inv_Fin_system.Init_inv_Fin)
     apply assumption
-   apply(blast intro: Init_inv_Fin_system.reachable_Fin)
+   apply (blast intro: Init_inv_Fin_system.reachable_Fin)
   apply simp
-  apply(fastforce dest: injD)
+  apply (fastforce dest: injD)
   done
 
 sublocale Init_inv_Fin_system \<subseteq> Init_Fin_system
-  apply(rule Init_inv_Fin_system_Init_Fin_system)
-  apply(unfold_locales)
+  apply (rule Init_inv_Fin_system_Init_Fin_system)
+  apply (unfold_locales)
   done
-
 
 
 section \<open>Non interference\<close>
@@ -427,60 +420,53 @@ locale noninterference_policy =
     "(x,schedDomain) \<in> policy \<Longrightarrow> x = schedDomain"
 begin
 
-abbreviation uwr2 :: "'s \<Rightarrow> 'd \<Rightarrow> 's \<Rightarrow> bool" ("(_/ \<sim>_\<sim>/ _)" [50,100,50] 1000)
-where
+abbreviation uwr2 :: "'s \<Rightarrow> 'd \<Rightarrow> 's \<Rightarrow> bool" ("(_/ \<sim>_\<sim>/ _)" [50,100,50] 1000) where
   "s \<sim>u\<sim> t \<equiv> (s,t) \<in> uwr u"
 
-abbreviation policy2 :: "'d \<Rightarrow> 'd \<Rightarrow> bool" (infix "\<leadsto>" 50)
-where
+abbreviation policy2 :: "'d \<Rightarrow> 'd \<Rightarrow> bool" (infix "\<leadsto>" 50) where
   "u \<leadsto> v \<equiv> (u,v) \<in> policy"
 
 lemma uwr_refl:
   "s \<sim>(u::'d)\<sim> s"
-  apply(cut_tac u=u in uwr_equiv_rel)
-  apply(clarsimp simp: equiv_def)
-  apply(blast dest: refl_onD)
+  apply (cut_tac u=u in uwr_equiv_rel)
+  apply (clarsimp simp: equiv_def)
+  apply (blast dest: refl_onD)
   done
 
 lemma uwr_sym:
   "x \<sim>(u::'d)\<sim> y \<Longrightarrow> y \<sim>u\<sim> x"
-  apply(cut_tac u=u in uwr_equiv_rel)
-  apply(clarsimp simp: equiv_def)
-  apply(blast dest: symD)
+  apply (cut_tac u=u in uwr_equiv_rel)
+  apply (clarsimp simp: equiv_def)
+  apply (blast dest: symD)
   done
 
 lemma uwr_trans:
-  "\<lbrakk>x \<sim>(u::'d)\<sim> y; y \<sim>u\<sim> z\<rbrakk> \<Longrightarrow> x \<sim>u\<sim> z"
-  apply(cut_tac u=u in uwr_equiv_rel)
-  apply(clarsimp simp: equiv_def)
-  apply(blast dest: transD)
+  "\<lbrakk> x \<sim>(u::'d)\<sim> y; y \<sim>u\<sim> z \<rbrakk> \<Longrightarrow> x \<sim>u\<sim> z"
+  apply (cut_tac u=u in uwr_equiv_rel)
+  apply (clarsimp simp: equiv_def)
+  apply (blast dest: transD)
   done
 
-definition sameFor_dom :: "'s \<Rightarrow> 'd set \<Rightarrow> 's \<Rightarrow> bool"  ("(_/ \<approx>_\<approx>/ _)" [50,100,50] 1000)
-where
- "s \<approx>us\<approx> t \<equiv> \<forall>u\<in>us. (s,t) \<in> uwr u"
+definition sameFor_dom :: "'s \<Rightarrow> 'd set \<Rightarrow> 's \<Rightarrow> bool"  ("(_/ \<approx>_\<approx>/ _)" [50,100,50] 1000) where
+  "s \<approx>us\<approx> t \<equiv> \<forall>u\<in>us. (s,t) \<in> uwr u"
 
 lemma sameFor_subset_dom: "\<lbrakk>s \<approx>(x::'d set)\<approx> t; y \<subseteq> x\<rbrakk> \<Longrightarrow> s \<approx>y\<approx> t"
-  by(fastforce simp: sameFor_dom_def)
-
+  by (fastforce simp: sameFor_dom_def)
 
 lemma sameFor_inter_domI: "s \<approx>(S::'d set)\<approx> t \<Longrightarrow> s \<approx>(S \<inter> B)\<approx> t"
-  by(auto simp: sameFor_dom_def)
-
+  by (auto simp: sameFor_dom_def)
 
 lemma sameFor_sym_dom:
   "s \<approx>(S::'d set)\<approx> t \<Longrightarrow> t \<approx>S\<approx> s"
-  by(auto simp: sameFor_dom_def uwr_sym)
+  by (auto simp: sameFor_dom_def uwr_sym)
 
 end
 
 
-
-
 subsection \<open>Non interference system\<close>
 
-locale noninterference_system = enabled_system A s0 +
-                                noninterference_policy dom uwr policy out schedDomain
+locale noninterference_system =
+  enabled_system A s0 + noninterference_policy dom uwr policy out schedDomain
   for A :: "('a,'s,'e) data_type"
   and s0 :: "'s"
   and dom :: "'e \<Rightarrow> 's \<Rightarrow> 'd"
@@ -492,289 +478,240 @@ begin
 
 (* The set of domains (which carry out actions in the list "as") which
  * may influence "u", assuming we start in state "s". *)
-primrec
- sources :: "'e list \<Rightarrow> 's \<Rightarrow> 'd \<Rightarrow> 'd set"
-where
- sources_Nil: "sources [] s u = {u}"|
- sources_Cons: "sources (a#as) s u = (\<Union>{sources as s' u| s'. (s,s') \<in> Step a}) \<union>
-      {w. w = dom a s \<and> (\<exists> v s'. dom a s \<leadsto> v \<and> (s,s') \<in> Step a \<and> v \<in> sources as s' u)}"
+primrec sources :: "'e list \<Rightarrow> 's \<Rightarrow> 'd \<Rightarrow> 'd set" where
+  sources_Nil: "sources [] s u = {u}"
+| sources_Cons: "sources (a#as) s u =
+    (\<Union>{sources as s' u| s'. (s,s') \<in> Step a}) \<union>
+    {w. w = dom a s \<and> (\<exists>v s'. dom a s \<leadsto> v \<and> (s,s') \<in> Step a \<and> v \<in> sources as s' u)}"
 
 declare sources_Nil [simp del]
 declare sources_Cons [simp del]
 
+definition obs_equiv :: "'s \<Rightarrow> 'e list \<Rightarrow> 's \<Rightarrow> 'e list \<Rightarrow> 'd \<Rightarrow> bool" where
+  "obs_equiv s as t bs d \<equiv>
+     \<forall>s' t'. s' \<in> execution A s as \<and> t' \<in> execution A t bs \<longrightarrow> out d s' = out d t'"
 
-
-definition obs_equiv :: "'s \<Rightarrow> 'e list \<Rightarrow> 's \<Rightarrow> 'e list \<Rightarrow> 'd \<Rightarrow> bool"
-where
-  "obs_equiv s as t bs d \<equiv> \<forall> s' t'. s' \<in> execution A s as \<and> t' \<in> execution A t bs \<longrightarrow>
-                out d s' = out d t'"
-
-
-definition uwr_equiv :: "'s \<Rightarrow> 'e list \<Rightarrow> 's \<Rightarrow> 'e list \<Rightarrow> 'd \<Rightarrow> bool"
-where
-  "uwr_equiv s as t bs d \<equiv> \<forall> s' t'. s' \<in> execution A s as \<and> t' \<in> execution A t bs \<longrightarrow>
-                s' \<sim>d\<sim> t'"
-
+definition uwr_equiv :: "'s \<Rightarrow> 'e list \<Rightarrow> 's \<Rightarrow> 'e list \<Rightarrow> 'd \<Rightarrow> bool" where
+  "uwr_equiv s as t bs d \<equiv>
+     \<forall>s' t'. s' \<in> execution A s as \<and> t' \<in> execution A t bs \<longrightarrow> s' \<sim>d\<sim> t'"
 
 
 text \<open>Nonleakage\<close>
-definition Nonleakage :: "bool"
-where
-  "Nonleakage \<equiv> \<forall>as s u t. reachable s \<and> reachable t \<longrightarrow>
-     s \<sim>schedDomain\<sim> t \<longrightarrow>
-     s \<approx>(sources as s u)\<approx> t \<longrightarrow> obs_equiv s as t as u"
+definition Nonleakage :: "bool" where
+  "Nonleakage \<equiv> \<forall>as s u t. reachable s \<and> reachable t
+                            \<longrightarrow> s \<sim>schedDomain\<sim> t
+                            \<longrightarrow> s \<approx>(sources as s u)\<approx> t
+                            \<longrightarrow> obs_equiv s as t as u"
+
 
 text \<open>A generalisation of Nonleakage.\<close>
-definition Nonleakage_gen :: "bool"
-where
-  "Nonleakage_gen \<equiv> \<forall>as s u t. reachable s \<and> reachable t \<longrightarrow>
-     s \<sim>schedDomain\<sim> t \<longrightarrow>
-       s \<approx>(sources as s u)\<approx> t \<longrightarrow> uwr_equiv s as t as u"
-
-
+definition Nonleakage_gen :: "bool" where
+  "Nonleakage_gen \<equiv>
+     \<forall>as s u t. reachable s \<and> reachable t
+                \<longrightarrow> s \<sim>schedDomain\<sim> t
+                \<longrightarrow> s \<approx>(sources as s u)\<approx> t
+                \<longrightarrow> uwr_equiv s as t as u"
 
 
 lemma uwr_equiv_sym:
   "uwr_equiv s as t bs u \<Longrightarrow> uwr_equiv t bs s as u"
-  apply(fastforce simp: uwr_equiv_def uwr_sym)
-  done
+  by (fastforce simp: uwr_equiv_def uwr_sym)
 
 lemma uwr_equiv_trans:
-  "\<lbrakk>reachable t; uwr_equiv s as t bs x; uwr_equiv t bs u cs x\<rbrakk> \<Longrightarrow> uwr_equiv s as u cs x"
-  apply(clarsimp simp: uwr_equiv_def)
-  apply(cut_tac s=t and js=bs in reachable_enabled)
+  "\<lbrakk> reachable t; uwr_equiv s as t bs x; uwr_equiv t bs u cs x \<rbrakk>
+     \<Longrightarrow> uwr_equiv s as u cs x"
+  apply (clarsimp simp: uwr_equiv_def)
+  apply (cut_tac s=t and js=bs in reachable_enabled)
    apply assumption
-  apply(blast intro: uwr_trans)
+  apply (blast intro: uwr_trans)
   done
 
-primrec gen_purge :: "('e list \<Rightarrow> 's \<Rightarrow> 'd \<Rightarrow> 'd set) \<Rightarrow> 'd \<Rightarrow> 'e list \<Rightarrow> 's set \<Rightarrow> 'e list"
-where
-  Nil : "gen_purge source_func u []     ss = []" |
-  Cons: "gen_purge source_func u (a#as) ss =
-            (if (\<exists>s\<in>ss. dom a s \<in> source_func (a#as) s u) then
-               a#gen_purge source_func u as (\<Union>s\<in>ss. {s'. (s,s') \<in> Step a})
-             else
-               gen_purge source_func u as ss)"
+primrec gen_purge :: "('e list \<Rightarrow> 's \<Rightarrow> 'd \<Rightarrow> 'd set) \<Rightarrow> 'd \<Rightarrow> 'e list \<Rightarrow> 's set \<Rightarrow> 'e list" where
+  Nil: "gen_purge source_func u [] ss = []"
+| Cons: "gen_purge source_func u (a#as) ss =
+           (if \<exists>s\<in>ss. dom a s \<in> source_func (a#as) s u
+            then a # gen_purge source_func u as (\<Union>s\<in>ss. {s'. (s,s') \<in> Step a})
+            else gen_purge source_func u as ss)"
 
-
-
-definition ipurge
-where
- "ipurge \<equiv> gen_purge sources"
+definition ipurge where
+  "ipurge \<equiv> gen_purge sources"
 
 lemma ipurge_Nil:
   "ipurge u [] ss = []"
-  by(auto simp: ipurge_def)
-
-lemma ipurge_Cons:
-  "ipurge u (a#as) ss =
-     (if (\<exists> s\<in>ss. dom a s \<in> sources (a#as) s u) then
-         a#ipurge u as (\<Union>s\<in>ss. {s'. (s,s') \<in> Step a})
-      else
-         ipurge u as ss)"
   by (auto simp: ipurge_def)
 
+lemma ipurge_Cons:
+  "ipurge u (a#as) ss = (if (\<exists>s\<in>ss. dom a s \<in> sources (a#as) s u)
+                         then a#ipurge u as (\<Union>s\<in>ss. {s'. (s,s') \<in> Step a})
+                         else ipurge u as ss)"
+  by (auto simp: ipurge_def)
 
 lemma gen_purge_shortens:
   "length (gen_purge sf u as ss) \<le> length as"
-  apply(induct as arbitrary: ss)
-   apply(simp)
-  apply(clarsimp)
-  apply(rule le_trans)
+  apply (induct as arbitrary: ss; clarsimp)
+  apply (rule le_trans)
    apply assumption
   apply simp
   done
 
-
-
-
 lemma INT_cong':
-  assumes a: "\<And> x. Q x \<Longrightarrow> P x = P' x"
-  shows
-  "\<Inter>{P x|x. Q x} = \<Inter>{P' x|x. Q x}"
-  apply (auto simp: a)
-  done
+  assumes a: "\<And>x. Q x \<Longrightarrow> P x = P' x"
+  shows "\<Inter>{P x|x. Q x} = \<Inter>{P' x|x. Q x}"
+  by (auto simp: a)
 
 
 text \<open>Standard Noninterference\<close>
-
-definition Noninterference :: "bool"
-where
- "Noninterference \<equiv>
-  \<forall> u as s. reachable s \<longrightarrow>
-         (obs_equiv s as s (ipurge u as {s}) u)"
+definition Noninterference :: bool where
+ "Noninterference \<equiv> \<forall>u as s. reachable s \<longrightarrow> (obs_equiv s as s (ipurge u as {s}) u)"
 
 
 text \<open>Strong Noninterference\<close>
-definition Noninterference_strong :: "bool"
-where
- "Noninterference_strong \<equiv>
-  \<forall> u as bs s. reachable s \<longrightarrow>
-         (ipurge u as {s}) = (ipurge u bs {s}) \<longrightarrow>
-         (obs_equiv s as s bs u)"
-
+definition Noninterference_strong :: bool where
+  "Noninterference_strong \<equiv> \<forall>u as bs s. reachable s
+                                         \<longrightarrow> ipurge u as {s} = ipurge u bs {s}
+                                         \<longrightarrow> obs_equiv s as s bs u"
 
 
 lemma obs_equiv_sym:
   "obs_equiv s as t bs u \<Longrightarrow> obs_equiv t bs s as u"
-  apply(clarsimp simp: obs_equiv_def)
-  done
+  by (clarsimp simp: obs_equiv_def)
 
 lemma obs_equiv_trans:
-  "\<lbrakk>reachable t; obs_equiv s as t bs u; obs_equiv t bs x cs u\<rbrakk> \<Longrightarrow> obs_equiv s as x cs u"
-  apply(clarsimp simp: obs_equiv_def)
-  apply(cut_tac s=t and js=bs in reachable_enabled, assumption, blast)
+  "\<lbrakk> reachable t; obs_equiv s as t bs u; obs_equiv t bs x cs u \<rbrakk>
+     \<Longrightarrow> obs_equiv s as x cs u"
+  apply (clarsimp simp: obs_equiv_def)
+  apply (cut_tac s=t and js=bs in reachable_enabled, assumption, blast)
   done
 
 lemma Noninterference_Noninterference_strong:
-  "\<lbrakk>Noninterference\<rbrakk> \<Longrightarrow> Noninterference_strong"
-  apply(clarsimp simp: Noninterference_def Noninterference_strong_def)
-  apply(drule_tac x=u in spec)
-  apply(frule_tac x=as in spec, drule_tac x=s in spec)
-  apply(drule_tac x=bs in spec, drule_tac x=s in spec)
+  "Noninterference \<Longrightarrow> Noninterference_strong"
+  apply (clarsimp simp: Noninterference_def Noninterference_strong_def)
+  apply (drule_tac x=u in spec)
+  apply (frule_tac x=as in spec, drule_tac x=s in spec)
+  apply (drule_tac x=bs in spec, drule_tac x=s in spec)
   apply clarsimp
-  apply(rule obs_equiv_trans)
+  apply (rule obs_equiv_trans)
     apply assumption
    apply assumption
-  apply(erule obs_equiv_sym)
+  apply (erule obs_equiv_sym)
   done
 
 
-text \<open>Noninfluence -- the combination of Noninterference and
-   Nonleakage.
-
-   We add the assumption about equivalence wrt the scheduler's domain, as
-   is common in e.g. GVW.\<close>
-definition Noninfluence  :: "bool"
-where
+text \<open>
+  Noninfluence -- the combination of Noninterference and Nonleakage.
+  We add the assumption about equivalence wrt the scheduler's domain, as
+  is common in e.g. GVW.
+\<close>
+definition Noninfluence :: bool where
  "Noninfluence \<equiv>
-  \<forall> u as s t. reachable s \<and> reachable t \<longrightarrow>
-      s \<approx>(sources as s u)\<approx> t \<longrightarrow>  s \<sim>schedDomain\<sim> t \<longrightarrow>
-         obs_equiv s as t (ipurge u as {t}) u"
-
-
-
+    \<forall>u as s t. reachable s \<and> reachable t
+               \<longrightarrow> s \<approx>(sources as s u)\<approx> t
+               \<longrightarrow> s \<sim>schedDomain\<sim> t
+               \<longrightarrow> obs_equiv s as t (ipurge u as {t}) u"
 
 definition Noninfluence_strong  :: "bool"
 where
- "Noninfluence_strong \<equiv>
-  \<forall> u as bs s t. reachable s  \<and> reachable t \<longrightarrow>
-      s \<approx>(sources as s u)\<approx> t \<longrightarrow>  s \<sim>schedDomain\<sim> t \<longrightarrow>
-         ipurge u as {s} = ipurge u bs {s} \<longrightarrow>
-         obs_equiv s as t bs u"
-
-
+ "Noninfluence_strong \<equiv> \<forall>u as bs s t. reachable s \<and> reachable t
+                                      \<longrightarrow> s \<approx>(sources as s u)\<approx> t
+                                      \<longrightarrow> s \<sim>schedDomain\<sim> t
+                                      \<longrightarrow> ipurge u as {s} = ipurge u bs {s}
+                                      \<longrightarrow> obs_equiv s as t bs u"
 
 
 lemma notin_policyI:
-  "\<lbrakk>dom a s \<notin> sources (a # list) s u; \<exists> s'. (s,s') \<in> Step a \<and> ua \<in> sources list s' u\<rbrakk> \<Longrightarrow>
-   (dom a s,ua) \<notin> policy"
-  apply(clarsimp simp: sources_Cons)
-  done
-
+  "\<lbrakk> dom a s \<notin> sources (a # list) s u; \<exists>s'. (s,s') \<in> Step a \<and> ua \<in> sources list s' u \<rbrakk>
+     \<Longrightarrow> (dom a s,ua) \<notin> policy"
+  by (clarsimp simp: sources_Cons)
 
 lemma Noninfluence_strong_Noninterference_strong:
   "Noninfluence_strong \<Longrightarrow> Noninterference_strong"
-  apply(clarsimp simp: Noninfluence_strong_def Noninterference_strong_def)
-  apply(drule_tac x=u in spec, drule_tac x=as in spec, drule_tac x=bs in spec)
-  apply(fastforce simp: sameFor_dom_def uwr_refl)
+  apply (clarsimp simp: Noninfluence_strong_def Noninterference_strong_def)
+  apply (drule_tac x=u in spec, drule_tac x=as in spec, drule_tac x=bs in spec)
+  apply (fastforce simp: sameFor_dom_def uwr_refl)
   done
 
 lemma Noninfluence_strong_Nonleakage:
   "Noninfluence_strong \<Longrightarrow> Nonleakage"
-  apply(clarsimp simp: Noninfluence_strong_def Nonleakage_def)
-  done
+  by (clarsimp simp: Noninfluence_strong_def Nonleakage_def)
+
 
 text \<open>This stronger condition is needed
    to make the induction proof work for Noninterference. It can be viewed
    as a generalisation of Noninfluence; hence its name here.
 \<close>
-definition Noninfluence_gen :: "bool"
-where
- "Noninfluence_gen \<equiv>
-  \<forall> u as s ts. reachable s \<and> (\<forall> t \<in> ts. reachable t) \<longrightarrow>
-      (\<forall>t \<in> ts. s \<approx>(sources as s u)\<approx> t) \<longrightarrow>  (\<forall>t \<in> ts. s \<sim>schedDomain\<sim> t) \<longrightarrow>
-         (\<forall>t \<in> ts. uwr_equiv s as t (ipurge u as ts) u)"
+definition Noninfluence_gen :: bool where
+  "Noninfluence_gen \<equiv> \<forall>u as s ts. reachable s \<and> (\<forall>t \<in> ts. reachable t)
+                                   \<longrightarrow> (\<forall>t \<in> ts. s \<approx>(sources as s u)\<approx> t)
+                                   \<longrightarrow> (\<forall>t \<in> ts. s \<sim>schedDomain\<sim> t)
+                                   \<longrightarrow> (\<forall>t \<in> ts. uwr_equiv s as t (ipurge u as ts) u)"
 
-definition Noninfluence_uwr  :: "bool"
-where
- "Noninfluence_uwr \<equiv>
-  \<forall> u as s t. reachable s \<and> reachable t \<longrightarrow>
-      s \<approx>(sources as s u)\<approx> t \<longrightarrow>  s \<sim>schedDomain\<sim> t \<longrightarrow>
-         uwr_equiv s as t (ipurge u as {t}) u"
+definition Noninfluence_uwr  :: bool where
+  "Noninfluence_uwr \<equiv> \<forall>u as s t. reachable s \<and> reachable t
+                                  \<longrightarrow> s \<approx>(sources as s u)\<approx> t
+                                  \<longrightarrow> s \<sim>schedDomain\<sim> t
+                                  \<longrightarrow> uwr_equiv s as t (ipurge u as {t}) u"
 
-definition Noninfluence_strong_uwr :: "bool"
-where
- "Noninfluence_strong_uwr \<equiv>
-  \<forall> u as bs s t. reachable s  \<and> reachable t \<longrightarrow>
-      s \<approx>(sources as s u)\<approx> t \<longrightarrow>  s \<sim>schedDomain\<sim> t \<longrightarrow>
-         ipurge u as {s} = ipurge u bs {s} \<longrightarrow>
-         uwr_equiv s as t bs u"
+definition Noninfluence_strong_uwr :: bool where
+  "Noninfluence_strong_uwr \<equiv> \<forall>u as bs s t. reachable s \<and> reachable t
+                                            \<longrightarrow> s \<approx>(sources as s u)\<approx> t
+                                            \<longrightarrow> s \<sim>schedDomain\<sim> t
+                                            \<longrightarrow> ipurge u as {s} = ipurge u bs {s}
+                                            \<longrightarrow> uwr_equiv s as t bs u"
 
+definition output_consistent :: bool where
+  "output_consistent \<equiv> \<forall>u s s'. s \<sim>u\<sim> s'  \<longrightarrow> (out u s = out u s')"
 
-
-
-definition output_consistent :: "bool"
-where
-  "output_consistent \<equiv> \<forall> u s s'. s \<sim>u\<sim> s'  \<longrightarrow> (out u s = out u s')"
-
-definition confidentiality_u :: "bool"
-where
-  "confidentiality_u \<equiv> \<forall> a u s t.  reachable s \<and> reachable t \<longrightarrow>
-    s \<sim>schedDomain\<sim> t \<longrightarrow>
-    ((dom a s \<leadsto> u) \<longrightarrow> s \<sim>dom a s\<sim> t) \<longrightarrow>
-      s \<sim>u\<sim> t \<longrightarrow>
-      (\<forall> s' t'. (s,s') \<in> Step a \<and> (t,t') \<in> Step a \<longrightarrow>
-        s' \<sim>u\<sim> t')"
+definition confidentiality_u :: bool where
+  "confidentiality_u \<equiv> \<forall>a u s t. reachable s \<and> reachable t
+                                  \<longrightarrow> s \<sim>schedDomain\<sim> t
+                                  \<longrightarrow> ((dom a s \<leadsto> u) \<longrightarrow> s \<sim>dom a s\<sim> t)
+                                  \<longrightarrow> s \<sim>u\<sim> t
+                                  \<longrightarrow> (\<forall>s' t'. (s,s') \<in> Step a \<and> (t,t') \<in> Step a \<longrightarrow> s' \<sim>u\<sim> t')"
 
 lemma no_domain_visible_nondeterminism:
-  "\<lbrakk>confidentiality_u; reachable s; (s,s') \<in> Step a; (s,s'') \<in> Step a\<rbrakk> \<Longrightarrow> s' \<sim>d\<sim> s''"
-  apply(clarsimp simp: confidentiality_u_def)
-  apply(fastforce intro: uwr_refl)
+  "\<lbrakk> confidentiality_u; reachable s; (s,s') \<in> Step a; (s,s'') \<in> Step a \<rbrakk>
+     \<Longrightarrow> s' \<sim>d\<sim> s''"
+  apply (clarsimp simp: confidentiality_u_def)
+  apply (fastforce intro: uwr_refl)
   done
 
-definition integrity_u :: "bool"
-where
-  "integrity_u \<equiv> \<forall> a u s. reachable  s \<longrightarrow>
-   (dom a s,u) \<notin> policy  \<longrightarrow>
-   (\<forall> s'. (s,s') \<in> Step a \<longrightarrow> s \<sim>u\<sim> s')"
+definition integrity_u :: bool where
+  "integrity_u \<equiv>
+     \<forall>a u s. reachable s \<longrightarrow> (dom a s,u) \<notin> policy \<longrightarrow> (\<forall>s'. (s,s') \<in> Step a \<longrightarrow> s \<sim>u\<sim> s')"
 
 (*<*)
 (* integrity_u actually guarantees this (seemingly) stronger condition *)
-definition integrity_u_more :: "bool"
-where
-  "integrity_u_more \<equiv> \<forall> a u s. reachable s \<longrightarrow>
-   (dom a s,u) \<notin> policy \<longrightarrow>
-   (\<forall> s' t. s \<sim>u\<sim> t \<and> (s,s') \<in> Step a \<longrightarrow> s' \<sim>u\<sim> t)"
+definition integrity_u_more :: bool where
+  "integrity_u_more \<equiv> \<forall>a u s. reachable s
+                               \<longrightarrow> (dom a s,u) \<notin> policy
+                               \<longrightarrow> (\<forall>s' t. s \<sim>u\<sim> t \<and> (s,s') \<in> Step a \<longrightarrow> s' \<sim>u\<sim> t)"
 
 lemma integrity_u_more:
   "integrity_u \<Longrightarrow> integrity_u_more"
-  apply(clarsimp simp: integrity_u_more_def integrity_u_def)
-  apply(blast dest: uwr_sym uwr_trans)
+  apply (clarsimp simp: integrity_u_more_def integrity_u_def)
+  apply (blast dest: uwr_sym uwr_trans)
   done
 (*>*)
 
 lemma integrity_uD:
-  "\<lbrakk>integrity_u; reachable s; (dom a s,u) \<notin> policy;
-    s \<sim>u\<sim> t; (s,s') \<in> Step a\<rbrakk> \<Longrightarrow>
-   s' \<sim>u\<sim> t"
-  apply(drule integrity_u_more)
-  apply(simp add: integrity_u_more_def)
+  "\<lbrakk> integrity_u; reachable s; (dom a s,u) \<notin> policy; s \<sim>u\<sim> t; (s,s') \<in> Step a \<rbrakk>
+     \<Longrightarrow> s' \<sim>u\<sim> t"
+  apply (drule integrity_u_more)
+  apply (simp add: integrity_u_more_def)
   done
-
-
-
 
 text \<open>
   A weaker version of @{prop confidentiality_u} that, with
   @{prop integrity_u}, implies it.
 \<close>
-definition confidentiality_u_weak
-where
-  "confidentiality_u_weak \<equiv> \<forall> a u s t.  reachable s \<and> reachable t \<longrightarrow>
-    s \<sim>schedDomain\<sim> t \<longrightarrow> dom a s \<leadsto> u \<longrightarrow> s \<sim>(dom a s)\<sim> t \<longrightarrow>
-      s \<sim>u\<sim> t \<longrightarrow>
-        (\<forall> s' t'. (s,s') \<in> Step a \<and> (t,t') \<in> Step a \<longrightarrow> s' \<sim>u\<sim> t')"
+definition confidentiality_u_weak where
+  "confidentiality_u_weak \<equiv> \<forall>a u s t. reachable s \<and> reachable t
+                                       \<longrightarrow> s \<sim>schedDomain\<sim> t
+                                       \<longrightarrow> dom a s \<leadsto> u
+                                       \<longrightarrow> s \<sim>(dom a s)\<sim> t
+                                       \<longrightarrow> s \<sim>u\<sim> t
+                                       \<longrightarrow> (\<forall>s' t'. (s,s') \<in> Step a \<and> (t,t') \<in> Step a
+                                                    \<longrightarrow> s' \<sim>u\<sim> t')"
 
 lemma confidentiality_u_confidentiality_u_weak:
   "confidentiality_u \<Longrightarrow> confidentiality_u_weak"
@@ -783,112 +720,108 @@ lemma confidentiality_u_confidentiality_u_weak:
   done
 
 lemma impCE':
-  "\<lbrakk>P \<longrightarrow> Q; \<lbrakk>P; Q\<rbrakk> \<Longrightarrow> R; \<not> P \<Longrightarrow> R\<rbrakk> \<Longrightarrow> R"
-  apply auto
-  done
+  "\<lbrakk> P \<longrightarrow> Q; \<lbrakk>P; Q\<rbrakk> \<Longrightarrow> R; \<not> P \<Longrightarrow> R \<rbrakk> \<Longrightarrow> R"
+  by auto
 
 lemma confidentiality_u_weak:
-  "\<lbrakk>confidentiality_u_weak; integrity_u\<rbrakk> \<Longrightarrow>
-  confidentiality_u"
-  apply(clarsimp simp: confidentiality_u_def)
-  apply(erule impCE')
-   apply(subst (asm) confidentiality_u_weak_def, blast)
-  apply(frule integrity_uD, simp+)
-  apply(drule_tac s=t and t="s'" in integrity_uD)
+  "\<lbrakk> confidentiality_u_weak; integrity_u \<rbrakk>
+     \<Longrightarrow> confidentiality_u"
+  apply (clarsimp simp: confidentiality_u_def)
+  apply (erule impCE')
+   apply (subst (asm) confidentiality_u_weak_def, blast)
+  apply (frule integrity_uD, simp+)
+  apply (drule_tac s=t and t="s'" in integrity_uD)
       apply assumption
-     apply(drule_tac e=a in schedIncludesCurrentDom)
+     apply (drule_tac e=a in schedIncludesCurrentDom)
      apply simp
-    apply(blast intro: uwr_sym)
+    apply (blast intro: uwr_sym)
    apply assumption
-  apply(erule uwr_sym)
+  apply (erule uwr_sym)
   done
 
 lemma obs_equivI:
-  "\<lbrakk>output_consistent; uwr_equiv s as t bs ob\<rbrakk> \<Longrightarrow> obs_equiv s as t bs ob"
-  apply(clarsimp simp: obs_equiv_def)
-  apply(auto simp: uwr_equiv_def output_consistent_def)
+  "\<lbrakk> output_consistent; uwr_equiv s as t bs ob \<rbrakk> \<Longrightarrow> obs_equiv s as t bs ob"
+  apply (clarsimp simp: obs_equiv_def)
+  apply (auto simp: uwr_equiv_def output_consistent_def)
   done
 
 lemma Noninfluence_uwr_Noninfluence:
-  "\<lbrakk>output_consistent; Noninfluence_uwr\<rbrakk> \<Longrightarrow> Noninfluence"
-  apply(clarsimp simp: Noninfluence_def)
-  apply(erule obs_equivI)
-  apply(auto simp: Noninfluence_uwr_def)
+  "\<lbrakk> output_consistent; Noninfluence_uwr \<rbrakk> \<Longrightarrow> Noninfluence"
+  apply (clarsimp simp: Noninfluence_def)
+  apply (erule obs_equivI)
+  apply (auto simp: Noninfluence_uwr_def)
   done
 
 lemma Noninfluence_strong_uwr_Noninfluence_strong:
-  "\<lbrakk>output_consistent; Noninfluence_strong_uwr\<rbrakk> \<Longrightarrow> Noninfluence_strong"
-  apply(clarsimp simp: Noninfluence_strong_def)
-  apply(erule obs_equivI)
-  apply(auto simp: Noninfluence_strong_uwr_def)
+  "\<lbrakk> output_consistent; Noninfluence_strong_uwr \<rbrakk> \<Longrightarrow> Noninfluence_strong"
+  apply (clarsimp simp: Noninfluence_strong_def)
+  apply (erule obs_equivI)
+  apply (auto simp: Noninfluence_strong_uwr_def)
   done
 
 lemma sched_equiv_preserved:
-  "\<lbrakk>confidentiality_u;  reachable s; reachable t;
-   s \<sim>schedDomain\<sim> t; (s,s') \<in> Step a; (t,t') \<in> Step a\<rbrakk> \<Longrightarrow>
-   s' \<sim>schedDomain\<sim> t'"
-  apply(case_tac "dom a s = schedDomain")
-   apply(subst (asm) confidentiality_u_def)
-   apply(drule_tac x=a in spec)
-   apply(drule_tac x=schedDomain in spec)
-   apply(drule_tac x=s in spec)
-   apply(drule_tac x=t in spec)
+  "\<lbrakk> confidentiality_u; reachable s; reachable t;
+     s \<sim>schedDomain\<sim> t; (s,s') \<in> Step a; (t,t') \<in> Step a \<rbrakk>
+     \<Longrightarrow> s' \<sim>schedDomain\<sim> t'"
+  apply (case_tac "dom a s = schedDomain")
+   apply (subst (asm) confidentiality_u_def)
+   apply (drule_tac x=a in spec)
+   apply (drule_tac x=schedDomain in spec)
+   apply (drule_tac x=s in spec)
+   apply (drule_tac x=t in spec)
    apply simp
-  apply(subst (asm) confidentiality_u_def)
-  apply(blast intro: schedNotGlobalChannel)
+  apply (subst (asm) confidentiality_u_def)
+  apply (blast intro: schedNotGlobalChannel)
   done
 
 lemma sched_equiv_preserved_left:
-  "\<lbrakk>integrity_u; s \<sim>schedDomain\<sim> t;
-    dom a s \<noteq> schedDomain; (s,s') \<in> Step a; reachable s\<rbrakk> \<Longrightarrow>
-    s' \<sim>schedDomain\<sim> t"
-  apply(blast intro: integrity_uD schedNotGlobalChannel)
-  done
+  "\<lbrakk> integrity_u; s \<sim>schedDomain\<sim> t;
+     dom a s \<noteq> schedDomain; (s,s') \<in> Step a; reachable s \<rbrakk>
+     \<Longrightarrow> s' \<sim>schedDomain\<sim> t"
+  by (blast intro: integrity_uD schedNotGlobalChannel)
 
 lemma Noninfluence_gen_Noninterference:
-  "\<lbrakk>output_consistent; Noninfluence_gen\<rbrakk> \<Longrightarrow> Noninterference"
-  apply(clarsimp simp: Noninterference_def Noninfluence_gen_def)
-  apply(erule_tac x=u in allE)
-  apply(erule_tac x=as in allE)
-  apply(erule_tac x=s in allE)
-  apply(erule_tac x="{s}" in allE)
-  apply(clarsimp simp: sameFor_dom_def uwr_refl)
-  apply(blast intro: obs_equivI)
+  "\<lbrakk> output_consistent; Noninfluence_gen \<rbrakk> \<Longrightarrow> Noninterference"
+  apply (clarsimp simp: Noninterference_def Noninfluence_gen_def)
+  apply (erule_tac x=u in allE)
+  apply (erule_tac x=as in allE)
+  apply (erule_tac x=s in allE)
+  apply (erule_tac x="{s}" in allE)
+  apply (clarsimp simp: sameFor_dom_def uwr_refl)
+  apply (blast intro: obs_equivI)
   done
 
 lemma Noninfluence_gen_Noninfluence:
-  "\<lbrakk>output_consistent; Noninfluence_gen\<rbrakk> \<Longrightarrow> Noninfluence"
-  apply(clarsimp simp: Noninfluence_def Noninfluence_gen_def)
-  apply(erule_tac x=u in allE)
-  apply(erule_tac x=as in allE)
-  apply(erule_tac x=s in allE)
-  apply(erule_tac x="{t}" in allE)
-  apply(blast intro: obs_equivI)
+  "\<lbrakk> output_consistent; Noninfluence_gen \<rbrakk> \<Longrightarrow> Noninfluence"
+  apply (clarsimp simp: Noninfluence_def Noninfluence_gen_def)
+  apply (erule_tac x=u in allE)
+  apply (erule_tac x=as in allE)
+  apply (erule_tac x=s in allE)
+  apply (erule_tac x="{t}" in allE)
+  apply (blast intro: obs_equivI)
   done
 
 lemma Noninfluence_gen_Noninfluence_uwr:
-  "\<lbrakk>Noninfluence_gen\<rbrakk> \<Longrightarrow> Noninfluence_uwr"
-  apply(clarsimp simp: Noninfluence_uwr_def Noninfluence_gen_def)
-  done
+  "Noninfluence_gen \<Longrightarrow> Noninfluence_uwr"
+  by (clarsimp simp: Noninfluence_uwr_def Noninfluence_gen_def)
 
 lemma Noninfluence_gen_Noninterference_strong:
-  "\<lbrakk>output_consistent; Noninfluence_gen\<rbrakk> \<Longrightarrow> Noninterference_strong"
-  apply(rule Noninterference_Noninterference_strong)
-  apply(blast intro: Noninfluence_gen_Noninterference)
+  "\<lbrakk> output_consistent; Noninfluence_gen \<rbrakk> \<Longrightarrow> Noninterference_strong"
+  apply (rule Noninterference_Noninterference_strong)
+  apply (blast intro: Noninfluence_gen_Noninterference)
   done
 
-
 end
+
 
 subsection \<open>Noninterference on enabled Step system : unwinding system\<close>
 
 locale enabled_Step_system = enabled_system A s0 + Step_system A s0
   for A :: "('a,'s,'e) data_type" and s0 :: "'s"
 
-
 (* we define the unwinding conditions for any system *)
-locale unwinding_system = enabled_Step_system A s0 +
-                          noninterference_policy dom uwr policy out schedDomain
+locale unwinding_system =
+  enabled_Step_system A s0 + noninterference_policy dom uwr policy out schedDomain
   for A :: "('a,'s,'e) data_type"
   and s0 :: "'s"
   and dom :: "'e \<Rightarrow> 's \<Rightarrow> 'd"
@@ -897,436 +830,408 @@ locale unwinding_system = enabled_Step_system A s0 +
   and out :: "'d \<Rightarrow> 's \<Rightarrow> 'p"
   and schedDomain :: "'d"
 
-sublocale unwinding_system \<subseteq> noninterference_system
-  apply(unfold_locales)
-  done
+sublocale unwinding_system \<subseteq> noninterference_system by unfold_locales
 
 context unwinding_system begin
 
-
-
-
 lemma sources_refl:
   "reachable s \<Longrightarrow> u \<in> sources as s u"
-  apply(induct as arbitrary: s)
-   apply(simp add: sources_Nil)
-  apply(simp add: sources_Cons)
-  apply(frule_tac a=a in enabled_Step)
+  apply (induct as arbitrary: s)
+   apply (simp add: sources_Nil)
+  apply (simp add: sources_Cons)
+  apply (frule_tac a=a in enabled_Step)
   apply (auto simp: reachable_Step)
   done
 
-
-
 lemma schedDomain_in_sources_Cons:
-  "reachable s \<Longrightarrow> dom a s = schedDomain \<Longrightarrow> dom a s \<in> sources (a#as) s u"
-  apply(unfold sources_Cons)
-  apply(erule ssubst)
-  apply(rule UnI2)
-  apply(clarsimp)
-  apply(rule_tac x=u in exI)
-  apply(safe)
-   apply(rule schedFlowsToAll)
-  apply(frule_tac a=a in enabled_Step)
-  apply(fastforce dest: sources_refl reachable_Step)
+  "\<lbrakk> reachable s; dom a s = schedDomain \<rbrakk>
+     \<Longrightarrow> dom a s \<in> sources (a#as) s u"
+  apply (unfold sources_Cons)
+  apply (erule ssubst)
+  apply (rule UnI2)
+  apply (clarsimp)
+  apply (rule_tac x=u in exI)
+  apply (safe)
+   apply (rule schedFlowsToAll)
+  apply (frule_tac a=a in enabled_Step)
+  apply (fastforce dest: sources_refl reachable_Step)
   done
-
-
 
 lemma sources_eq':
   "confidentiality_u \<and> s \<sim>schedDomain\<sim> t \<and> reachable s \<and> reachable t
    \<longrightarrow> sources as s u = sources as t u"
-  proof (induct as arbitrary: s t)
+proof (induct as arbitrary: s t)
   case Nil show ?case
-   apply(simp add: sources_Nil)
-   done
-  next
+    by (simp add: sources_Nil)
+next
   case (Cons a as) show ?case
-  apply(clarsimp simp: sources_Cons)
-  apply(rule un_eq)
-   apply(simp only: Union_eq, simp only: UNION_eq[symmetric])
-   apply(rule Un_eq, clarsimp)
-     apply(metis "Cons.hyps"[rule_format] sched_equiv_preserved reachable_Step)
-    apply(fastforce intro: enabled_Step)
-   apply(fastforce intro: enabled_Step)
-  apply(clarsimp simp: schedIncludesCurrentDom)
-  apply(rule Collect_cong)
-  apply(rule conj_cong, rule refl)
-  apply(rule iff_exI)
-  apply(metis "Cons.hyps"[rule_format] sched_equiv_preserved reachable_Step enabled_Step)
-  done
-  qed
-
+    apply (clarsimp simp: sources_Cons)
+    apply (rule un_eq)
+     apply (simp only: Union_eq, simp only: UNION_eq[symmetric])
+     apply (rule Un_eq, clarsimp)
+       apply (metis "Cons.hyps"[rule_format] sched_equiv_preserved reachable_Step)
+      apply (fastforce intro: enabled_Step)
+     apply (fastforce intro: enabled_Step)
+    apply (clarsimp simp: schedIncludesCurrentDom)
+    apply (rule Collect_cong)
+    apply (rule conj_cong, rule refl)
+    apply (rule iff_exI)
+    apply (metis "Cons.hyps"[rule_format] sched_equiv_preserved reachable_Step enabled_Step)
+    done
+qed
 
 lemma sources_eq:
-  "\<lbrakk>confidentiality_u; s \<sim>schedDomain\<sim> t; reachable s; reachable t\<rbrakk> \<Longrightarrow>
-  sources as s u = sources as t u"
-  by(rule sources_eq'[rule_format], simp)
-
+  "\<lbrakk> confidentiality_u; s \<sim>schedDomain\<sim> t; reachable s; reachable t \<rbrakk>
+     \<Longrightarrow> sources as s u = sources as t u"
+  by (rule sources_eq'[rule_format], simp)
 
 lemma sameFor_sources_dom:
-  "\<lbrakk>s \<approx>(sources (a#as) s u)\<approx> t; dom a s \<leadsto> x; x \<in> sources as s' u; (s,s') \<in> Step a\<rbrakk> \<Longrightarrow>
-   s \<sim>(dom a s)\<sim> t"
-  apply(simp add: sameFor_dom_def)
-  apply(erule bspec)
-  apply(subst sources_Cons)
-  apply(rule UnI2)
+  "\<lbrakk> s \<approx>(sources (a#as) s u)\<approx> t; dom a s \<leadsto> x; x \<in> sources as s' u; (s,s') \<in> Step a \<rbrakk>
+     \<Longrightarrow> s \<sim>(dom a s)\<sim> t"
+  apply (simp add: sameFor_dom_def)
+  apply (erule bspec)
+  apply (subst sources_Cons)
+  apply (rule UnI2)
   apply blast
   done
 
 lemma sources_unwinding_step:
-  "\<lbrakk>s \<approx>(sources (a#as) s u)\<approx> t; s \<sim>schedDomain\<sim> t; confidentiality_u;
-    (s,s') \<in> Step a; (t,t') \<in> Step a; reachable s; reachable t\<rbrakk>  \<Longrightarrow>
-    s' \<approx>(sources as s' u)\<approx> t'"
-  apply(clarsimp simp: sameFor_dom_def sources_Cons)
-  apply(subst (asm) confidentiality_u_def)
-  apply(drule_tac x=a in spec)
-  apply(drule_tac x=ua in spec)
-  apply(drule_tac x=s in spec)
-  apply(drule_tac x=t in spec)
-  apply(fastforce intro: sameFor_sources_dom)
+  "\<lbrakk> s \<approx>(sources (a#as) s u)\<approx> t; s \<sim>schedDomain\<sim> t; confidentiality_u;
+     (s,s') \<in> Step a; (t,t') \<in> Step a; reachable s; reachable t \<rbrakk>
+     \<Longrightarrow> s' \<approx>(sources as s' u)\<approx> t'"
+  apply (clarsimp simp: sameFor_dom_def sources_Cons)
+  apply (subst (asm) confidentiality_u_def)
+  apply (drule_tac x=a in spec)
+  apply (drule_tac x=ua in spec)
+  apply (drule_tac x=s in spec)
+  apply (drule_tac x=t in spec)
+  apply (fastforce intro: sameFor_sources_dom)
   done
 
 lemma ipurge_eq'_helper:
-  "\<lbrakk>s \<in> ss; dom a s \<in> sources (a # as) s u; \<forall>s\<in>ts. dom a s \<notin> sources (a # as) s u;
-   (\<forall>s t. s \<in> ss \<and> t \<in> ts \<longrightarrow> s \<sim>schedDomain\<sim> t \<and> reachable s \<and> reachable t);
-   t \<in> ts; confidentiality_u\<rbrakk> \<Longrightarrow>
-  False"
-  apply(cut_tac s=s and t=t and as=as and u=u in sources_eq, simp+)
-  apply(clarsimp  simp: sources_Cons | safe)+
-  apply(rename_tac s')
-   apply(drule_tac x=t in bspec, simp)
+  "\<lbrakk> s \<in> ss; dom a s \<in> sources (a # as) s u; \<forall>s\<in>ts. dom a s \<notin> sources (a # as) s u;
+     (\<forall>s t. s \<in> ss \<and> t \<in> ts \<longrightarrow> s \<sim>schedDomain\<sim> t \<and> reachable s \<and> reachable t);
+     t \<in> ts; confidentiality_u \<rbrakk>
+     \<Longrightarrow> False"
+  apply (cut_tac s=s and t=t and as=as and u=u in sources_eq, simp+)
+  apply (clarsimp  simp: sources_Cons | safe)+
+   apply (rename_tac s')
+   apply (drule_tac x=t in bspec, simp)
    apply clarsimp
-   apply(cut_tac s=t in enabled_Step, simp)
-   apply(erule exE, rename_tac t')
-   apply(drule_tac x="sources as t' u" in spec)
-   apply(cut_tac s=s' and t=t' and u=u in sources_eq, simp+)
-      apply(fastforce elim: sched_equiv_preserved)
-     apply(fastforce intro: reachable_Step)
-    apply(fastforce intro: reachable_Step)
-   apply(fastforce simp: schedIncludesCurrentDom)
-  apply(drule_tac x=t in bspec, simp)
+   apply (cut_tac s=t in enabled_Step, simp)
+   apply (erule exE, rename_tac t')
+   apply (drule_tac x="sources as t' u" in spec)
+   apply (cut_tac s=s' and t=t' and u=u in sources_eq, simp+)
+      apply (fastforce elim: sched_equiv_preserved)
+     apply (fastforce intro: reachable_Step)
+    apply (fastforce intro: reachable_Step)
+   apply (fastforce simp: schedIncludesCurrentDom)
+  apply (drule_tac x=t in bspec, simp)
   apply clarsimp
-  apply(rename_tac v s')
-  apply(drule_tac x=v in spec, erule impE, fastforce simp: schedIncludesCurrentDom)
-  apply(cut_tac s=t in enabled_Step[where a=a], simp, clarsimp, rename_tac t')
-  apply(cut_tac s=s' and t=t' and u=u in sources_eq, simp+)
-     apply(fastforce elim: sched_equiv_preserved)
-    apply(fastforce intro: reachable_Step)
-   apply(fastforce intro: reachable_Step)
-  apply(fastforce simp: schedIncludesCurrentDom)
+  apply (rename_tac v s')
+  apply (drule_tac x=v in spec, erule impE, fastforce simp: schedIncludesCurrentDom)
+  apply (cut_tac s=t in enabled_Step[where a=a], simp, clarsimp, rename_tac t')
+  apply (cut_tac s=s' and t=t' and u=u in sources_eq, simp+)
+     apply (fastforce elim: sched_equiv_preserved)
+    apply (fastforce intro: reachable_Step)
+   apply (fastforce intro: reachable_Step)
+  apply (fastforce simp: schedIncludesCurrentDom)
   done
 
-
-
 lemma ipurge_eq':
-  "(\<forall> s t. s\<in>ss \<and> t\<in>ts \<longrightarrow> s \<sim>schedDomain\<sim> t \<and> reachable s \<and> reachable t) \<and>
-   (\<exists> s. s \<in> ss) \<and> (\<exists> t. t \<in> ts) \<and> confidentiality_u
-    \<longrightarrow> ipurge u as ss = ipurge u as ts"
-  proof (induct as arbitrary: ss ts)
+  "(\<forall>s t. s\<in>ss \<and> t\<in>ts \<longrightarrow> s \<sim>schedDomain\<sim> t \<and> reachable s \<and> reachable t) \<and>
+   (\<exists>s. s \<in> ss) \<and> (\<exists>t. t \<in> ts) \<and> confidentiality_u
+   \<longrightarrow> ipurge u as ss = ipurge u as ts"
+proof (induct as arbitrary: ss ts)
   case Nil show ?case
-   apply(simp add: ipurge_def)
-   done
-  next
+    apply (simp add: ipurge_def)
+    done
+next
   case (Cons a as) show ?case
-   apply(clarsimp simp: ipurge_Cons schedIncludesCurrentDom)
-   apply(intro conjI impI)
-      apply(rule "Cons.hyps"[rule_format])
+    apply (clarsimp simp: ipurge_Cons schedIncludesCurrentDom)
+    apply (intro conjI impI)
+       apply (rule "Cons.hyps"[rule_format])
+       apply clarsimp
+       apply (metis sched_equiv_preserved reachable_Step enabled_Step)
       apply clarsimp
-      apply(metis sched_equiv_preserved reachable_Step enabled_Step)
+      apply (drule ipurge_eq'_helper, simp+)[1]
      apply clarsimp
-     apply(drule ipurge_eq'_helper, simp+)[1]
-    apply clarsimp
-    apply(drule ipurge_eq'_helper, (simp add: uwr_sym)+)[1]
-   apply(rule "Cons.hyps"[rule_format], auto)
-   done
-  qed
+     apply (drule ipurge_eq'_helper, (simp add: uwr_sym)+)[1]
+    apply (rule "Cons.hyps"[rule_format], auto)
+    done
+qed
 
 lemma ipurge_eq:
-  "\<lbrakk>s \<sim>schedDomain\<sim> t; reachable s; reachable t;
-    confidentiality_u\<rbrakk> \<Longrightarrow>
-   ipurge u as {s} = ipurge u as {t}"
-  by(rule ipurge_eq'[rule_format], simp)
+  "\<lbrakk> s \<sim>schedDomain\<sim> t; reachable s; reachable t; confidentiality_u \<rbrakk>
+     \<Longrightarrow> ipurge u as {s} = ipurge u as {t}"
+  by (rule ipurge_eq'[rule_format], simp)
 
 lemma Noninfluence_uwr_Noninfluence_strong_uwr:
-  "\<lbrakk>confidentiality_u; Noninfluence_uwr\<rbrakk> \<Longrightarrow> Noninfluence_strong_uwr"
-  apply(clarsimp simp: Noninfluence_uwr_def Noninfluence_strong_uwr_def)
-  apply(frule_tac s=s and t=t and as=as and u=u in ipurge_eq)
+  "\<lbrakk> confidentiality_u; Noninfluence_uwr \<rbrakk> \<Longrightarrow> Noninfluence_strong_uwr"
+  apply (clarsimp simp: Noninfluence_uwr_def Noninfluence_strong_uwr_def)
+  apply (frule_tac s=s and t=t and as=as and u=u in ipurge_eq)
      apply assumption+
-  apply(frule_tac s=s and t=t and as=bs and u=u in ipurge_eq)
+  apply (frule_tac s=s and t=t and as=bs and u=u in ipurge_eq)
      apply assumption+
   apply clarsimp
-  apply(drule_tac x=u in spec)
-  apply(frule_tac x=as in spec)
-  apply(drule_tac x=s in spec, drule_tac x=t in spec)
-  apply(drule_tac x=bs in spec)
-  apply(drule_tac x=t in spec, drule_tac x=t in spec)
+  apply (drule_tac x=u in spec)
+  apply (frule_tac x=as in spec)
+  apply (drule_tac x=s in spec, drule_tac x=t in spec)
+  apply (drule_tac x=bs in spec)
+  apply (drule_tac x=t in spec, drule_tac x=t in spec)
   apply clarsimp
-  apply(rule_tac t=t in uwr_equiv_trans)
+  apply (rule_tac t=t in uwr_equiv_trans)
     apply assumption
    apply assumption
-  apply(rule uwr_equiv_sym)
-  apply(clarsimp simp: sameFor_dom_def uwr_refl)
+  apply (rule uwr_equiv_sym)
+  apply (clarsimp simp: sameFor_dom_def uwr_refl)
   done
 
 lemma Noninfluence_Noninfluence_strong:
-  "\<lbrakk>confidentiality_u; Noninfluence\<rbrakk> \<Longrightarrow> Noninfluence_strong"
-  apply(clarsimp simp: Noninfluence_def Noninfluence_strong_def)
-  apply(frule_tac s=s and t=t and as=as and u=u in ipurge_eq)
+  "\<lbrakk> confidentiality_u; Noninfluence \<rbrakk> \<Longrightarrow> Noninfluence_strong"
+  apply (clarsimp simp: Noninfluence_def Noninfluence_strong_def)
+  apply (frule_tac s=s and t=t and as=as and u=u in ipurge_eq)
      apply assumption+
-  apply(frule_tac s=s and t=t and as=bs and u=u in ipurge_eq)
+  apply (frule_tac s=s and t=t and as=bs and u=u in ipurge_eq)
      apply assumption+
   apply clarsimp
-  apply(drule_tac x=u in spec)
-  apply(frule_tac x=as in spec)
-  apply(drule_tac x=s in spec, drule_tac x=t in spec)
-  apply(drule_tac x=bs in spec)
-  apply(drule_tac x=t in spec, drule_tac x=t in spec)
+  apply (drule_tac x=u in spec)
+  apply (frule_tac x=as in spec)
+  apply (drule_tac x=s in spec, drule_tac x=t in spec)
+  apply (drule_tac x=bs in spec)
+  apply (drule_tac x=t in spec, drule_tac x=t in spec)
   apply clarsimp
-  apply(rule_tac t=t in obs_equiv_trans)
+  apply (rule_tac t=t in obs_equiv_trans)
     apply assumption
    apply assumption
-  apply(rule obs_equiv_sym)
-  apply(clarsimp simp: sameFor_dom_def uwr_refl)
+  apply (rule obs_equiv_sym)
+  apply (clarsimp simp: sameFor_dom_def uwr_refl)
   done
-
 
 lemma dom_in_sources_Cons:
-  "\<lbrakk>confidentiality_u; reachable s; reachable t;
-    s \<approx>(sources (a#as) s u)\<approx> t; s \<sim>schedDomain\<sim> t;
-    (dom a s \<in> sources (a#as) s u)\<rbrakk> \<Longrightarrow>
-    (dom a t \<in> sources (a#as) t u)"
-  apply(subgoal_tac "dom a s = dom a t")
-   apply(fastforce dest: sources_eq)
-  apply(blast intro: schedIncludesCurrentDom)
+  "\<lbrakk> confidentiality_u; reachable s; reachable t; s \<approx>(sources (a#as) s u)\<approx> t;
+     s \<sim>schedDomain\<sim> t; (dom a s \<in> sources (a#as) s u) \<rbrakk>
+     \<Longrightarrow> (dom a t \<in> sources (a#as) t u)"
+  apply (subgoal_tac "dom a s = dom a t")
+   apply (fastforce dest: sources_eq)
+  apply (blast intro: schedIncludesCurrentDom)
   done
-
-
 
 lemma uwr_equiv_Cons_bothI:
-   "\<lbrakk>reachable s; reachable t;
-     \<forall> s' t'. (s,s') \<in> Step a \<and> (t,t') \<in> Step b \<longrightarrow> uwr_equiv s' as t' bs u\<rbrakk> \<Longrightarrow>
-    uwr_equiv s (a # as) t (b # bs) u"
-  apply(clarsimp simp: uwr_equiv_def)
-  apply(clarsimp simp: execution_Run)
-  apply(fastforce simp: execution_Run reachable_Step)
-  done
+  "\<lbrakk> reachable s; reachable t;
+      \<forall>s' t'. (s,s') \<in> Step a \<and> (t,t') \<in> Step b \<longrightarrow> uwr_equiv s' as t' bs u \<rbrakk>
+     \<Longrightarrow> uwr_equiv s (a # as) t (b # bs) u"
+  by (fastforce simp: uwr_equiv_def execution_Run reachable_Step)
 
 lemma uwr_equiv_Cons_leftI:
-   "\<lbrakk>reachable s; \<forall> s'. (s,s') \<in> Step a \<longrightarrow> uwr_equiv s' as t bs u\<rbrakk> \<Longrightarrow>
-    uwr_equiv s (a # as) t bs u"
-  by(fastforce simp: uwr_equiv_def execution_Run reachable_Step)
-
+  "\<lbrakk> reachable s; \<forall>s'. (s,s') \<in> Step a \<longrightarrow> uwr_equiv s' as t bs u \<rbrakk>
+     \<Longrightarrow> uwr_equiv s (a # as) t bs u"
+  by (fastforce simp: uwr_equiv_def execution_Run reachable_Step)
 
 lemma notin_policyI':
-  "\<lbrakk>reachable s;
-    dom a s \<notin> sources (a # list) s u; (s,s') \<in> Step a; ua \<in> sources list s' u\<rbrakk> \<Longrightarrow>
-   (dom a s,ua) \<notin> policy"
-  apply(rule notin_policyI)
-  apply auto
+  "\<lbrakk> reachable s; dom a s \<notin> sources (a # list) s u; (s,s') \<in> Step a; ua \<in> sources list s' u \<rbrakk>
+     \<Longrightarrow> (dom a s,ua) \<notin> policy"
+  apply (rule notin_policyI)
+   apply auto
   done
 
 lemma sources_eq_Step:
-  "\<lbrakk>integrity_u; confidentiality_u; reachable s; (s,s') \<in> Step a; dom a s \<noteq> schedDomain\<rbrakk> \<Longrightarrow>
-   (sources as s' u) = (sources as s u)"
-  apply(rule sources_eq, simp+)
-    apply(rule_tac t=s and s=s and a=a in sched_equiv_preserved_left,
-          (simp add: uwr_refl reachable_Step)+)
+  "\<lbrakk> integrity_u; confidentiality_u; reachable s; (s,s') \<in> Step a; dom a s \<noteq> schedDomain \<rbrakk>
+     \<Longrightarrow> (sources as s' u) = (sources as s u)"
+  apply (rule sources_eq, simp+)
+    apply (rule_tac t=s and s=s and a=a in sched_equiv_preserved_left)
+        apply (auto simp add: uwr_refl reachable_Step)
   done
 
 lemma sources_equiv_preserved_left:
-  "\<lbrakk>integrity_u; confidentiality_u; reachable s; reachable t; s \<sim>schedDomain\<sim> t;
-    dom a s \<notin> sources (a#as) s u; s \<approx>sources (a#as) s u\<approx> t; (s,s') \<in> Step a; dom a s \<noteq> schedDomain\<rbrakk>
-    \<Longrightarrow> s' \<approx>sources as s' u\<approx> t"
-  apply(clarsimp simp: sameFor_dom_def)
-  apply(rename_tac v)
-  apply(case_tac "(dom a s, v) \<in> policy")
-   apply(fastforce simp: sources_Cons)
-  apply(fastforce dest: integrity_uD simp: sources_Cons)
+  "\<lbrakk> integrity_u; confidentiality_u; reachable s; reachable t; s \<sim>schedDomain\<sim> t;
+     dom a s \<notin> sources (a#as) s u; s \<approx>sources (a#as) s u\<approx> t; (s,s') \<in> Step a;
+     dom a s \<noteq> schedDomain \<rbrakk>
+     \<Longrightarrow> s' \<approx>sources as s' u\<approx> t"
+  apply (clarsimp simp: sameFor_dom_def)
+  apply (rename_tac v)
+  apply (case_tac "(dom a s, v) \<in> policy")
+   apply (fastforce simp: sources_Cons)
+  apply (fastforce dest: integrity_uD simp: sources_Cons)
   done
 
 lemma Noninfluence_gen:
-  "\<lbrakk>confidentiality_u; integrity_u\<rbrakk> \<Longrightarrow> Noninfluence_gen"
-  apply(subst Noninfluence_gen_def)
-  apply(intro allI)
-  proof -
+  "\<lbrakk> confidentiality_u; integrity_u \<rbrakk> \<Longrightarrow> Noninfluence_gen"
+  apply (subst Noninfluence_gen_def)
+  apply (intro allI)
+proof -
   assume conf: "confidentiality_u"
   assume integ: "integrity_u"
   fix u as s ts
-  show "reachable s \<and> Ball ts reachable \<longrightarrow>
-          Ball ts (sameFor_dom s (sources as s u)) \<longrightarrow> (\<forall>t\<in>ts. s \<sim>schedDomain\<sim> t)
-          \<longrightarrow> (\<forall>t\<in>ts. uwr_equiv s as t (ipurge u as ts) u)"
-    proof(induct as arbitrary: s ts)
+  show "reachable s \<and> Ball ts reachable
+        \<longrightarrow> Ball ts (sameFor_dom s (sources as s u))
+        \<longrightarrow> (\<forall>t\<in>ts. s \<sim>schedDomain\<sim> t)
+        \<longrightarrow> (\<forall>t\<in>ts. uwr_equiv s as t (ipurge u as ts) u)"
+  proof(induct as arbitrary: s ts)
     case Nil
     show ?case
-      apply(clarsimp simp: sameFor_dom_def ipurge_Nil sources_Nil uwr_equiv_def)
-      apply(clarsimp simp: execution_Run)
+      apply (clarsimp simp: sameFor_dom_def ipurge_Nil sources_Nil uwr_equiv_def)
+      apply (clarsimp simp: execution_Run)
       done
-    next
+  next
     case (Cons a as)
     show ?case
-  apply(clarsimp simp: ipurge_Cons | safe)+
-   apply(rule uwr_equiv_Cons_bothI)
-     apply assumption
-    apply blast
-   apply(clarify)
-   apply(rename_tac ta tb s' tb')
-   apply(rule Cons.hyps[rule_format])
-      apply(blast intro: reachable_Step)
-     apply(clarsimp)
-     apply(rename_tac tc' tc)
-     using conf apply(rule_tac s=s and t=tc and a=a in sources_unwinding_step, simp+)[1]
-    apply(clarsimp, rename_tac tc' tc)
-    apply(rule sched_equiv_preserved[OF conf], (auto simp: sources_refl))[1]
-   apply blast
-  apply(rename_tac ta)
-  apply(rule uwr_equiv_Cons_leftI, blast)
-  apply(clarsimp, rename_tac s')
-  apply(case_tac "dom a s = schedDomain")
-   apply(cut_tac s=s and a=a and as=as and u=u in schedDomain_in_sources_Cons, assumption+)
-   apply(metis schedIncludesCurrentDom sources_eq[OF conf])
-  apply(rule Cons.hyps[rule_format])
-     apply(blast intro: reachable_Step)
-    apply(rename_tac tb)
-    apply(rule_tac a=a in sources_equiv_preserved_left[OF integ conf], simp+)
-       apply(fastforce simp: schedIncludesCurrentDom sources_eq[OF conf])
-      apply blast
-     apply assumption
-    apply assumption
-   apply(rule_tac s=s and a=a in sched_equiv_preserved_left[OF integ], simp+)
-  done
+      apply (clarsimp simp: ipurge_Cons | safe)+
+       apply (rule uwr_equiv_Cons_bothI)
+         apply assumption
+        apply blast
+       apply (clarify)
+       apply (rename_tac ta tb s' tb')
+       apply (rule Cons.hyps[rule_format])
+          apply (blast intro: reachable_Step)
+         apply (clarsimp)
+         apply (rename_tac tc' tc)
+      using conf apply (rule_tac s=s and t=tc and a=a in sources_unwinding_step, simp+)[1]
+        apply (clarsimp, rename_tac tc' tc)
+        apply (rule sched_equiv_preserved[OF conf], (auto simp: sources_refl))[1]
+       apply blast
+      apply (rename_tac ta)
+      apply (rule uwr_equiv_Cons_leftI, blast)
+      apply (clarsimp, rename_tac s')
+      apply (case_tac "dom a s = schedDomain")
+       apply (cut_tac s=s and a=a and as=as and u=u in schedDomain_in_sources_Cons, assumption+)
+       apply (metis schedIncludesCurrentDom sources_eq[OF conf])
+      apply (rule Cons.hyps[rule_format])
+         apply (blast intro: reachable_Step)
+        apply (rename_tac tb)
+        apply (rule_tac a=a in sources_equiv_preserved_left[OF integ conf], simp+)
+           apply (fastforce simp: schedIncludesCurrentDom sources_eq[OF conf])
+          apply blast
+         apply assumption
+        apply assumption
+       apply (rule_tac s=s and a=a in sched_equiv_preserved_left[OF integ], simp+)
+      done
   qed
-  qed
+qed
 
 lemma Nonleakage_gen:
-  "\<lbrakk>confidentiality_u\<rbrakk> \<Longrightarrow> Nonleakage_gen"
-  apply(subst Nonleakage_gen_def)
-  apply(rule allI)
-  apply(induct_tac as)
-   apply(simp add: sources_Nil uwr_equiv_def execution_Run sameFor_dom_def)
-  apply(clarsimp)
-  apply(rule uwr_equiv_Cons_bothI)
+  "confidentiality_u \<Longrightarrow> Nonleakage_gen"
+  apply (subst Nonleakage_gen_def)
+  apply (rule allI)
+  apply (induct_tac as)
+   apply (simp add: sources_Nil uwr_equiv_def execution_Run sameFor_dom_def)
+  apply (clarsimp)
+  apply (rule uwr_equiv_Cons_bothI)
     apply assumption
    apply assumption
   apply clarsimp
-  apply(drule_tac x=s' in spec, drule_tac x=u in spec, drule_tac x=t' in spec)
-  apply(clarsimp simp: reachable_Step)
-  apply(erule impE)
-   apply(blast intro: sched_equiv_preserved)
-  apply(erule mp)
-  apply(blast intro: sources_unwinding_step)
+  apply (drule_tac x=s' in spec, drule_tac x=u in spec, drule_tac x=t' in spec)
+  apply (clarsimp simp: reachable_Step)
+  apply (erule impE)
+   apply (blast intro: sched_equiv_preserved)
+  apply (erule mp)
+  apply (blast intro: sources_unwinding_step)
   done
 
-
-
 lemma Noninterference:
-  "\<lbrakk>confidentiality_u_weak; output_consistent; integrity_u\<rbrakk> \<Longrightarrow>
-   Noninterference"
-  apply(rule Noninfluence_gen_Noninterference)
+  "\<lbrakk> confidentiality_u_weak; output_consistent; integrity_u \<rbrakk>
+     \<Longrightarrow> Noninterference"
+  apply (rule Noninfluence_gen_Noninterference)
    apply assumption
-  apply(blast intro: Noninfluence_gen confidentiality_u_weak)
+  apply (blast intro: Noninfluence_gen confidentiality_u_weak)
   done
 
 lemma Noninterference_strong:
-  "\<lbrakk>confidentiality_u_weak; output_consistent; integrity_u\<rbrakk> \<Longrightarrow>
-   Noninterference_strong"
-  apply(rule Noninfluence_gen_Noninterference_strong)
+  "\<lbrakk> confidentiality_u_weak; output_consistent; integrity_u \<rbrakk>
+     \<Longrightarrow> Noninterference_strong"
+  apply (rule Noninfluence_gen_Noninterference_strong)
    apply assumption
-  apply(blast intro: Noninfluence_gen confidentiality_u_weak)
+  apply (blast intro: Noninfluence_gen confidentiality_u_weak)
   done
 
-
-
 lemma Noninfluence:
-  "\<lbrakk>confidentiality_u_weak; output_consistent; integrity_u\<rbrakk> \<Longrightarrow>
-   Noninfluence"
-  apply(rule Noninfluence_gen_Noninfluence)
+  "\<lbrakk> confidentiality_u_weak; output_consistent; integrity_u \<rbrakk>
+     \<Longrightarrow> Noninfluence"
+  apply (rule Noninfluence_gen_Noninfluence)
    apply assumption
-  apply(blast intro: Noninfluence_gen confidentiality_u_weak)
+  apply (blast intro: Noninfluence_gen confidentiality_u_weak)
   done
 
 lemma Noninfluence_strong:
-  "\<lbrakk>confidentiality_u_weak; output_consistent; integrity_u\<rbrakk> \<Longrightarrow>
-   Noninfluence_strong"
-  apply(rule Noninfluence_Noninfluence_strong)
-   apply(blast intro: confidentiality_u_weak)
-  apply(blast intro: Noninfluence)
+  "\<lbrakk> confidentiality_u_weak; output_consistent; integrity_u \<rbrakk>
+     \<Longrightarrow> Noninfluence_strong"
+  apply (rule Noninfluence_Noninfluence_strong)
+   apply (blast intro: confidentiality_u_weak)
+  apply (blast intro: Noninfluence)
   done
 
 
 lemma Noninfluence_uwr:
-  "\<lbrakk>confidentiality_u_weak; integrity_u\<rbrakk> \<Longrightarrow>
-   Noninfluence_uwr"
-  apply(rule Noninfluence_gen_Noninfluence_uwr)
-  apply(blast intro: Noninfluence_gen confidentiality_u_weak)
+  "\<lbrakk> confidentiality_u_weak; integrity_u \<rbrakk>
+     \<Longrightarrow> Noninfluence_uwr"
+  apply (rule Noninfluence_gen_Noninfluence_uwr)
+  apply (blast intro: Noninfluence_gen confidentiality_u_weak)
   done
 
 lemma Noninfluence_strong_uwr:
-  "\<lbrakk>confidentiality_u_weak; integrity_u\<rbrakk> \<Longrightarrow>
-   Noninfluence_strong_uwr"
-  apply(rule Noninfluence_uwr_Noninfluence_strong_uwr)
-   apply(blast intro: confidentiality_u_weak)
-  apply(blast intro: Noninfluence_uwr)
+  "\<lbrakk> confidentiality_u_weak; integrity_u \<rbrakk>
+     \<Longrightarrow> Noninfluence_strong_uwr"
+  apply (rule Noninfluence_uwr_Noninfluence_strong_uwr)
+   apply (blast intro: confidentiality_u_weak)
+  apply (blast intro: Noninfluence_uwr)
   done
 
 lemma sources_Step:
-  "\<lbrakk>reachable s; (dom a s, u) \<notin> policy\<rbrakk> \<Longrightarrow>
-  sources [a] s u = {u}"
-  apply(auto simp: sources_Cons sources_Nil enabled_Step dest: enabled_Step)
-  done
+  "\<lbrakk> reachable s; (dom a s, u) \<notin> policy \<rbrakk>
+     \<Longrightarrow> sources [a] s u = {u}"
+  by (auto simp: sources_Cons sources_Nil enabled_Step dest: enabled_Step)
 
 lemma sources_Step_2:
-  "\<lbrakk>reachable s; (dom a s, u) \<in> policy\<rbrakk> \<Longrightarrow>
-  sources [a] s u = {dom a s,u}"
-  apply(auto simp: sources_Cons sources_Nil enabled_Step dest: enabled_Step)
-  done
+  "\<lbrakk> reachable s; (dom a s, u) \<in> policy \<rbrakk>
+     \<Longrightarrow> sources [a] s u = {dom a s,u}"
+  by (auto simp: sources_Cons sources_Nil enabled_Step dest: enabled_Step)
 
 lemma execution_Nil:
   "reachable s \<Longrightarrow> execution A s [] = {s}"
-  apply(simp add: execution_Run)
-  done
+  by (simp add: execution_Run)
 
 lemma Noninfluence_gen_confidentiality_u_weak:
   "Noninfluence_gen \<Longrightarrow> confidentiality_u_weak"
-  apply(clarsimp simp: Noninfluence_gen_def confidentiality_u_weak_def)
-  apply(drule_tac x=u in spec, drule_tac x="[a]" in spec)
-  apply(drule_tac x=s in spec, drule_tac x="{t}" in spec)
-  apply(simp add: sources_Step_2 sameFor_dom_def uwr_equiv_def Step_def ipurge_Cons ipurge_Nil
-           split: if_splits
-             add: schedIncludesCurrentDom)
+  apply (clarsimp simp: Noninfluence_gen_def confidentiality_u_weak_def)
+  apply (drule_tac x=u in spec, drule_tac x="[a]" in spec)
+  apply (drule_tac x=s in spec, drule_tac x="{t}" in spec)
+  apply (simp add: sources_Step_2 sameFor_dom_def uwr_equiv_def Step_def
+                   ipurge_Cons ipurge_Nil schedIncludesCurrentDom
+            split: if_splits)
   done
 
 lemma Noninfluence_strong_uwr_confidentiality_u_weak:
   "Noninfluence_strong_uwr \<Longrightarrow> confidentiality_u_weak"
-  apply(clarsimp simp: Noninfluence_strong_uwr_def confidentiality_u_weak_def)
-  apply(drule_tac x=u in spec, drule_tac x="[a]" in spec, drule_tac x="[a]" in spec)
-  apply(drule_tac x=s in spec, drule_tac x=t in spec)
-  apply(simp add: sources_Step_2 sameFor_dom_def uwr_equiv_def Step_def)
+  apply (clarsimp simp: Noninfluence_strong_uwr_def confidentiality_u_weak_def)
+  apply (drule_tac x=u in spec, drule_tac x="[a]" in spec, drule_tac x="[a]" in spec)
+  apply (drule_tac x=s in spec, drule_tac x=t in spec)
+  apply (simp add: sources_Step_2 sameFor_dom_def uwr_equiv_def Step_def)
   done
 
 lemma Nonleakage_gen_confidentiality_u:
   "Nonleakage_gen \<Longrightarrow> confidentiality_u"
-  apply(clarsimp simp: Nonleakage_gen_def confidentiality_u_def)
-  apply(drule_tac x="[a]" in spec, drule_tac x=s in spec)
-  apply(drule_tac x=u in spec, drule_tac x=t in spec)
-  apply(case_tac "dom a s \<leadsto> u")
-   apply(simp add: sources_Step_2 uwr_equiv_def sameFor_dom_def Step_def)
-  apply(simp add: sources_Step uwr_equiv_def sameFor_dom_def Step_def)
+  apply (clarsimp simp: Nonleakage_gen_def confidentiality_u_def)
+  apply (drule_tac x="[a]" in spec, drule_tac x=s in spec)
+  apply (drule_tac x=u in spec, drule_tac x=t in spec)
+  apply (case_tac "dom a s \<leadsto> u")
+   apply (simp add: sources_Step_2 uwr_equiv_def sameFor_dom_def Step_def)
+  apply (simp add: sources_Step uwr_equiv_def sameFor_dom_def Step_def)
   done
 
 lemma Nonleakage_gen_equiv_confidentiality_u:
   "Nonleakage_gen = confidentiality_u"
-  apply(blast intro: Nonleakage_gen_confidentiality_u Nonleakage_gen)
-  done
+  by (blast intro: Nonleakage_gen_confidentiality_u Nonleakage_gen)
 
 lemma non_sched_doms_cannot_schedule:
-  "\<lbrakk>integrity_u; reachable s; dom a s \<noteq> schedDomain; (s,s') \<in> Step a\<rbrakk> \<Longrightarrow> s \<sim>schedDomain\<sim> s'"
-  apply(drule_tac u=schedDomain in integrity_uD)
+  "\<lbrakk> integrity_u; reachable s; dom a s \<noteq> schedDomain; (s,s') \<in> Step a \<rbrakk>
+     \<Longrightarrow> s \<sim>schedDomain\<sim> s'"
+  apply (drule_tac u=schedDomain in integrity_uD)
       apply assumption
-     apply(erule contrapos_nn)
-     apply(erule schedNotGlobalChannel)
-    apply(rule uwr_refl)
+     apply (erule contrapos_nn)
+     apply (erule schedNotGlobalChannel)
+    apply (rule uwr_refl)
    apply assumption
-  apply(erule uwr_sym)
+  apply (erule uwr_sym)
   done
 
 
@@ -1339,29 +1244,29 @@ text \<open>
    event) doesn't satisfy @{prop integrity_u}.
 \<close>
 lemma integrity_u_and_single_event_systems:
-  "\<lbrakk>integrity_u; reachable s; dom a s \<noteq> schedDomain; s' \<in> execution A s as;
-    \<forall> y::'e. y = a\<rbrakk> \<Longrightarrow> dom e s' \<noteq> schedDomain"
-  apply(frule_tac x=e in spec)
-  apply(erule ssubst)
-  apply(rule_tac P="\<lambda>x. x \<noteq> schedDomain" in subst[rotated])
+  "\<lbrakk> integrity_u; reachable s; dom a s \<noteq> schedDomain; s' \<in> execution A s as; \<forall>y. y = a \<rbrakk>
+     \<Longrightarrow> dom e s' \<noteq> schedDomain"
+  apply (frule_tac x=e in spec)
+  apply (erule ssubst)
+  apply (rule_tac P="\<lambda>x. x \<noteq> schedDomain" in subst[rotated])
    apply assumption
-  apply(induct as arbitrary: s s' a rule: rev_induct)
-   apply(simp add: execution_Run)
-  apply(simp add: execution_Run)
-  apply(drule Run_mid)
-  apply(erule exE, rename_tac t)
-  apply(drule_tac x=s in meta_spec)
-  apply(drule_tac x=t in meta_spec)
-  apply(drule_tac x=a in meta_spec)
+  apply (induct as arbitrary: s s' a rule: rev_induct)
+   apply (simp add: execution_Run)
+  apply (simp add: execution_Run)
+  apply (drule Run_mid)
+  apply (erule exE, rename_tac t)
+  apply (drule_tac x=s in meta_spec)
+  apply (drule_tac x=t in meta_spec)
+  apply (drule_tac x=a in meta_spec)
   apply simp
-  apply(rule schedIncludesCurrentDom)
-  apply(rule non_sched_doms_cannot_schedule)
+  apply (rule schedIncludesCurrentDom)
+  apply (rule non_sched_doms_cannot_schedule)
      apply assumption
-    apply(rule reachable_execution)
+    apply (rule reachable_execution)
      apply assumption
-    apply(fastforce simp: execution_Run)
+    apply (fastforce simp: execution_Run)
    apply assumption
-  apply(drule_tac x=x in spec)
+  apply (drule_tac x=x in spec)
   apply blast
   done
 
@@ -1372,31 +1277,30 @@ subsection \<open>Complete unwinding system\<close>
 
 text \<open>The unwinding conditions are not only sound but also complete when policy is reflexive\<close>
 locale complete_unwinding_system = unwinding_system +
-  assumes  policy_refl:
-  "(u,u) \<in> policy"
+  assumes policy_refl: "(u,u) \<in> policy"
 begin
 
 lemma Noninfluence_gen_integrity_u:
   "Noninfluence_gen \<Longrightarrow> integrity_u"
-  apply(clarsimp simp: Noninfluence_gen_def integrity_u_def)
-  apply(drule_tac x=u in spec, drule_tac x="[a]" in spec)
-  apply(drule_tac x=s in spec, drule_tac x="{s}" in spec)
-  apply(simp add: sources_Step sameFor_dom_def uwr_equiv_def Step_def ipurge_Cons ipurge_Nil
-           split: if_splits add: uwr_refl policy_refl execution_Nil uwr_sym)
+  apply (clarsimp simp: Noninfluence_gen_def integrity_u_def)
+  apply (drule_tac x=u in spec, drule_tac x="[a]" in spec)
+  apply (drule_tac x=s in spec, drule_tac x="{s}" in spec)
+  apply (simp add: sources_Step sameFor_dom_def uwr_equiv_def Step_def ipurge_Cons ipurge_Nil
+                   uwr_refl policy_refl execution_Nil uwr_sym
+            split: if_splits )
   done
-
 
 lemma Noninfluence_strong_uwr_integrity_u:
   "Noninfluence_strong_uwr \<Longrightarrow> integrity_u"
-  apply(clarsimp simp: Noninfluence_strong_uwr_def integrity_u_def)
-  apply(drule_tac x=u in spec, drule_tac x="[a]" in spec, drule_tac x="[]" in spec)
-  apply(drule_tac x=s in spec, drule_tac x=s in spec)
-  apply(simp add: sources_Step sameFor_dom_def uwr_refl uwr_equiv_def Step_def ipurge_Cons
-                  ipurge_Nil
-           split: if_splits)
-   apply(simp add: policy_refl)
-  apply(simp add: execution_Nil)
-  apply(blast intro: uwr_sym)
+  apply (clarsimp simp: Noninfluence_strong_uwr_def integrity_u_def)
+  apply (drule_tac x=u in spec, drule_tac x="[a]" in spec, drule_tac x="[]" in spec)
+  apply (drule_tac x=s in spec, drule_tac x=s in spec)
+  apply (simp add: sources_Step sameFor_dom_def uwr_refl
+                   uwr_equiv_def Step_def ipurge_Cons ipurge_Nil
+            split: if_splits)
+   apply (simp add: policy_refl)
+  apply (simp add: execution_Nil)
+  apply (blast intro: uwr_sym)
   done
 
 text \<open>
@@ -1407,14 +1311,14 @@ text \<open>
 \<close>
 lemma Noninfluence_gen_equiv_Noninfluence_strong_uwr:
   "Noninfluence_gen = Noninfluence_strong_uwr"
-  apply(rule iffI)
-   apply(rule Noninfluence_strong_uwr)
-    apply(erule Noninfluence_gen_confidentiality_u_weak)
-   apply(erule Noninfluence_gen_integrity_u)
-  apply(rule Noninfluence_gen)
-   apply(rule confidentiality_u_weak)
-    apply(erule Noninfluence_strong_uwr_confidentiality_u_weak)
-   apply(erule Noninfluence_strong_uwr_integrity_u)+
+  apply (rule iffI)
+   apply (rule Noninfluence_strong_uwr)
+    apply (erule Noninfluence_gen_confidentiality_u_weak)
+   apply (erule Noninfluence_gen_integrity_u)
+  apply (rule Noninfluence_gen)
+   apply (rule confidentiality_u_weak)
+    apply (erule Noninfluence_strong_uwr_confidentiality_u_weak)
+   apply (erule Noninfluence_strong_uwr_integrity_u)+
   done
 
 end
